proof/correctness/avx2/1024/MLKEM_W16_Rep.ec
@@ -1,127 +1,60 @@
 require import AllCore List Int IntDiv BitEncoding.
 from Jasmin require import JModel.
 from JazzEC require import Array256 Array1024 Array1536 Array4096.
-from Spec require import GFq Rq VecMat Serialization Correctness1024 EncDecCorrectness1024.
+from Spec require import GFq Rq Parameters VecMat Serialization Correctness EncDecCorrectness.
 require import MLKEMFCLib.
+require import MLKEM1024_prelude.
 import MLKEMFCLib1024.
 import Zq.
-import VecMat1024 PolyVec PolyMat Serialization1024 KMatrix.
+import VecMat PolyVec PolyMat Serialization KMatrix.
 import KMatrix.Matrix.
 import BitChunking BS2Int.
 
 op lift_polyvec (vec: W16.t Array1024.t) : polyvec =
-  Vector.offunv (fun i => lift_array256 (subarray256 vec i)).
+  KVec.init (fun i => lift_array256 (subarray256 vec i)).
 
 op lift_matrix( a : W16.t Array4096.t) : polymat =
-   Matrix.offunm (fun i j => subarray256 (subarray1024 (lift_array4096 a) i) j).
+   KMat.init (fun flat => subarray256 (subarray1024 (lift_array4096 a) (flat %/ kvec)) (flat %% kvec)).
 
 (* toipolyvec/lift_polyvec bridge (relocated from ref's MLKEM_InnerPKE.ec). *)
 lemma toipolivec_lift (_v : W16.t Array1024.t) :
-  toipolyvec (lift_polyvec _v) = map asint (lift_array1024 _v).
+  toipolyvec (lift_polyvec _v) = IPVec.init (fun idx => asint (lift_array1024 _v).[idx]).
 proof.
-rewrite /toipolyvec /lift_polyvec /lift_array1024 /fromarray256;congr => /=;rewrite tP => k kb.
-rewrite mapiE 1:/# /= initiE 1:/# /= /lift_array256 /subarray256.
-case (0<=k<256) => * /=.
-+ by rewrite getvE offunvE /= 1:/# mapiE 1:/# /= initiE 1:/# /=.
-case (256<=k<512) => * /=.
-+ by rewrite getvE offunvE /= 1:/# mapiE 1:/# /= initiE 1:/# /=.
-case (512<=k<768) => * /=.
-+ by rewrite getvE offunvE /= 1:/# mapiE 1:/# /= initiE 1:/# /=.
-by rewrite getvE offunvE /= 1:/# mapiE 1:/# /= initiE 1:/# /=.
-qed.
-
-(* Bound on decode (relocated from ref/MLKEM_Poly.ec, size-256 variant). *)
-lemma decode_range dfl (l : W8.t list) n :
-  1 < n <= 12 =>
-    size l = 256*n %/ 8 =>
-  size (decode n l) = 256 /\
-  (forall k, 0<=k<256 => 0<= nth dfl (decode n l) k <2^n).
-move => ? Hsl *.
-rewrite -andaE;split.
-+ rewrite /decode size_map size_chunk 1:/# size_BytesToBits Hsl /#.
-move => ? k kb.
-rewrite /decode.
-have := size_nth_chunk witness (BytesToBits l) k n; rewrite size_BytesToBits /= => H.
-rewrite (nth_map witness);1: by rewrite size_chunk 1:/# size_BytesToBits Hsl /#.
-split => *; 1: smt(BS2Int.bs2int_ge0).
-have ? : 8 * size l %/ n = 256; last by  smt(BS2Int.bs2int_le2Xs).
-by rewrite Hsl;smt().
-qed.
-
-(* polyvec variant of decode_range, 1024 *)
-lemma decode_range_vec dfl (l : W8.t list) n :
-  1 < n <= 12 =>
-    size l = 1024*n %/ 8 =>
-  size (decode n l) = 1024 /\
-  (forall k, 0<=k<1024 => 0<= nth dfl (decode n l) k <2^n).
-move => ? Hsl *.
-rewrite -andaE;split.
-+ rewrite /decode size_map size_chunk 1:/# size_BytesToBits Hsl /#.
-move => ? k kb.
-rewrite /decode.
-have := size_nth_chunk witness (BytesToBits l) k n; rewrite size_BytesToBits /= => H.
-rewrite (nth_map witness);1: by rewrite size_chunk 1:/# size_BytesToBits Hsl /#.
-split => *; 1: smt(BS2Int.bs2int_ge0).
-have ? : 8 * size l %/ n = 1024; last by  smt(BS2Int.bs2int_le2Xs).
-by rewrite Hsl;smt().
+have kv := kvec_val.
+rewrite /toipolyvec; apply IPVec.tP => idx ib.
+rewrite !IPVec.initiE 1,2:/# /=; congr.
+rewrite /lift_polyvec KVec.initiE 1:/#.
+rewrite /= /lift_array256 mapiE 1:/#.
+rewrite mapiE 1:/# /subarray256 initiE 1:/# /=.
+by have ->: 256 * (idx %/ 256) + idx %% 256 = idx by smt().
 qed.
 
 (* Spec-side bound on decoded 12-bit ints. *)
-lemma decode12_vec_bnd (a : W8.t Array1536.t) (k : int) :
+lemma decode12_vec_bnd (a : W8.t BytesPKVec.t) (k : int) :
   0 <= k < 1024 => 0 <= (decode12_vec a).[k] < 4096.
 proof.
-move => ?; rewrite /decode12_vec get_of_list 1:/# /decode (nth_map witness).
-+ by rewrite size_chunk 1:/# size_BytesToBits size_to_list //=.
+move => ?; have kv := kvec_val.
+rewrite /decode12_vec IPVec.get_of_list 1:/# /ByteDecode (nth_map witness).
++ rewrite size_chunk 1:/# size_BytesToBits size_to_list; smt().
 have := bs2int_le2Xs (nth witness (chunk 12 (BytesToBits (to_list a))) k).
-rewrite size_nth_chunk //=;1: by rewrite size_BytesToBits size_to_list //=.
+rewrite size_nth_chunk //=;1: by (rewrite size_BytesToBits size_to_list; smt()).
 by smt(bs2int_ge0).
 qed.
 
 op unlift_polyvec(a : polyvec) =
-   Array1024.init (fun i => W16.of_int (as_sint (a.[i %/ 256])%Vector.[i%%256])).
+   Array1024.init (fun i => W16.of_int (as_sint a.[i %/ 256].[i%%256])).
 
 lemma vector_unlift a :
     lift_polyvec (unlift_polyvec a) = a /\
     signed_bound1024_cxq (unlift_polyvec a) 0 1024 1.
 proof.
+have kv := kvec_val.
 split.
-+ rewrite /lift_vector /unlift_polyvec eq_vectorP => i ib.
-  rewrite offunvE //= /subarray256 /lift_array256 /= tP => k kb.
++ rewrite /unlift_polyvec; apply KVec.tP => i ib.
+  rewrite /lift_polyvec KVec.initiE 1:/# /= /subarray256 /lift_array256 /= tP => k kb.
   rewrite mapiE //= initiE //= initiE //= 1:/# /to_sint /smod /=.
-  rewrite !of_uintK /=; rewrite /as_sint qE /=.
-  by smt(rg_asint asintK).
-rewrite /unlift_vector /signed_bound1024_cxq => k kb; rewrite initiE //=.
-rewrite /to_sint /smod /= !of_uintK /= /as_sint qE /=.
-by smt(rg_asint).
+  rewrite !of_uintK /=; smt(rg_crepr as_sintK qE).
+rewrite /unlift_polyvec /signed_bound1024_cxq => k kb; rewrite initiE //=.
+rewrite /to_sint /smod /= !of_uintK /=; smt(rg_crepr qE).
 qed.
 
-lemma ofipolyvec_lift vi vw :
-  all (fun i => 0 <= i < 32768) vi =>
-  lift_array1024 vw = map incoeff vi =>
-  ofipolyvec vi = lift_polyvec vw.
-rewrite allP /= => ?.
-rewrite /lift_array1024 tP => H.
-rewrite /ofipolyvec /lift_polyvec !setvE /= eq_vectorP => r rb.
-rewrite !offunvE 1,2:/# /= !offunvK /vclamp /= /subarray256 /lift_array256.
-case(3 = r).
-+ move => r0; rewrite r0 /=.
-  rewrite tP => k kb; rewrite !mapiE 1,2:/#  /= !initiE 1,2:/# /=.
-  have := H (256*r+k) _;1:smt().
-  rewrite !mapiE /#.
-case(2 = r).
-+ move => r0?; rewrite r0 /= ifT 1:/#.
-  rewrite tP => k kb; rewrite !mapiE 1,2:/#  /= !initiE 1,2:/# /=.
-  have := H (256*r+k) _;1:smt().
-  rewrite !mapiE /#.
-case(1 = r).
-+ move => r0??; rewrite r0 /= ifT 1:/# ifT 1:/#.
-  rewrite tP => k kb; rewrite !mapiE 1,2:/#  /= !initiE 1,2:/# /=.
-  have := H (256*r+k) _;1:smt().
-  rewrite !mapiE /#.
-move => *.
-have -> /= : r= 0 by smt().
-rewrite !ifT 1..3:/#.
-rewrite tP => k kb; rewrite !mapiE 1,2:/#  /= !initiE 1,2:/# /=.
-have := H (256*r+k) _;1:smt().
-rewrite !mapiE /#.
-qed.
