proof/correctness/avx2/1024/NTT_avx2.ec
@@ -7,51 +7,19 @@ from JazzEC require import Array256 Array128 Array32 Array16 Array1024 Array4096
 require import MLKEMFCLib.
 import MLKEMFCLib1024.
 require import MLKEM_W16_Rep.
+require import MLKEM1024_prelude.
 require import NTT_Fq.
 require import AVX2_Ops.
 
-from Spec require import GFq Rq Serialization VecMat Correctness1024.
-import VecMat1024 Serialization1024.
+from Spec require import GFq Rq Serialization VecMat Correctness.
+import VecMat Serialization.
 
 import Zq IntOrder BitReverse.
 import PolyVec PolyMat.
+require import NTT_avx2_poly.
+
 theory NTT_Avx2.
 
-abbrev nttpack_idx = Array256.of_list witness
-  [0; 16; 32; 48; 64; 80; 96; 112; 1; 17; 33; 49; 65; 81; 97; 113;
-   2; 18; 34; 50; 66; 82; 98; 114; 3; 19; 35; 51; 67; 83; 99; 115;
-   4; 20; 36; 52; 68; 84; 100; 116; 5; 21; 37; 53; 69; 85; 101; 117;
-   6; 22; 38; 54; 70; 86; 102; 118; 7; 23; 39; 55; 71; 87; 103; 119;
-   8; 24; 40; 56; 72; 88; 104; 120; 9; 25; 41; 57; 73; 89; 105; 121;
-   10; 26; 42; 58; 74; 90; 106; 122; 11; 27; 43; 59; 75; 91; 107; 123;
-   12; 28; 44; 60; 76; 92; 108; 124; 13; 29; 45; 61; 77; 93; 109; 125;
-   14; 30; 46; 62; 78; 94; 110; 126; 15; 31; 47; 63; 79; 95; 111; 127;
-   128; 144; 160; 176; 192; 208; 224; 240; 129; 145; 161; 177; 193; 209; 225; 241;
-   130; 146; 162; 178; 194; 210; 226; 242; 131; 147; 163; 179; 195; 211; 227; 243;
-   132; 148; 164; 180; 196; 212; 228; 244; 133; 149; 165; 181; 197; 213; 229; 245;
-   134; 150; 166; 182; 198; 214; 230; 246; 135; 151; 167; 183; 199; 215; 231; 247;
-   136; 152; 168; 184; 200; 216; 232; 248; 137; 153; 169; 185; 201; 217; 233; 249;
-   138; 154; 170; 186; 202; 218; 234; 250; 139; 155; 171; 187; 203; 219; 235; 251;
-   140; 156; 172; 188; 204; 220; 236; 252; 141; 157; 173; 189; 205; 221; 237; 253;
-   142; 158; 174; 190; 206; 222; 238; 254; 143; 159; 175; 191; 207; 223; 239; 255].
-
-abbrev nttunpack_idx = Array256.of_list witness
-  [0; 8; 16; 24; 32; 40; 48; 56; 64; 72; 80; 88; 96; 104; 112; 120;
-   1; 9; 17; 25; 33; 41; 49; 57; 65; 73; 81; 89; 97; 105; 113; 121;
-   2; 10; 18; 26; 34; 42; 50; 58; 66; 74; 82; 90; 98; 106; 114; 122;
-   3; 11; 19; 27; 35; 43; 51; 59; 67; 75; 83; 91; 99; 107; 115; 123;
-   4; 12; 20; 28; 36; 44; 52; 60; 68; 76; 84; 92; 100; 108; 116; 124;
-   5; 13; 21; 29; 37; 45; 53; 61; 69; 77; 85; 93; 101; 109; 117; 125;
-   6; 14; 22; 30; 38; 46; 54; 62; 70; 78; 86; 94; 102; 110; 118; 126;
-   7; 15; 23; 31; 39; 47; 55; 63; 71; 79; 87; 95; 103; 111; 119; 127;
-   128; 136; 144; 152; 160; 168; 176; 184; 192; 200; 208; 216; 224; 232; 240; 248;
-   129; 137; 145; 153; 161; 169; 177; 185; 193; 201; 209; 217; 225; 233; 241; 249;
-   130; 138; 146; 154; 162; 170; 178; 186; 194; 202; 210; 218; 226; 234; 242; 250;
-   131; 139; 147; 155; 163; 171; 179; 187; 195; 203; 211; 219; 227; 235; 243; 251;
-   132; 140; 148; 156; 164; 172; 180; 188; 196; 204; 212; 220; 228; 236; 244; 252;
-   133; 141; 149; 157; 165; 173; 181; 189; 197; 205; 213; 221; 229; 237; 245; 253;
-   134; 142; 150; 158; 166; 174; 182; 190; 198; 206; 214; 222; 230; 238; 246; 254;
-   135; 143; 151; 159; 167; 175; 183; 191; 199; 207; 215; 223; 231; 239; 247; 255].
 
 abbrev shuffle8_idx = Array32.of_list witness
   [0; 1; 2; 3; 4; 5; 6; 7; 16; 17; 18; 19; 20; 21; 22; 23;
@@ -68,12 +36,6 @@ abbrev shuffle2_idx = Array32.of_list witness
 abbrev shuffle1_idx = Array32.of_list witness
   [0; 16; 2; 18; 4; 20; 6; 22; 8; 24; 10; 26; 12; 28; 14; 30;
    1; 17; 3; 19; 5; 21; 7; 23; 9; 25; 11; 27; 13; 29; 15; 31].
-
-op nttpack (rp : 'a Array256.t) : ('a Array256.t) = Array256.init (fun i => rp.[nttpack_idx.[i]])
-axiomatized by nttpackE.
-
-op nttunpack (rp: 'a Array256.t) : ('a Array256.t) = Array256.init (fun i => rp.[nttunpack_idx.[i]])
-axiomatized by nttunpackE.
 
 op shuf8 (a b: 'a Array16.t) : ('a Array16.t * 'a Array16.t) =
   let c = Array32.init (fun i => if 16 <= i then b.[i %% 16] else a.[i]) in
@@ -103,32 +65,6 @@ op shuf1 (a b: 'a Array16.t) : ('a Array16.t * 'a Array16.t) =
   let br = Array16.init (fun i => cr.[i + 16]) in
   (ar, br).
 
-lemma nttpack_idxK : all (fun i => nttpack_idx.[nttunpack_idx.[i]] = i) (iota_ 0 256)
-by rewrite -iotaredE /=.
-
-lemma nttunpack_idxK : all (fun i => nttunpack_idx.[nttpack_idx.[i]] = i) (iota_ 0 256)
-by rewrite -iotaredE /=.
-
-lemma nttpackK: cancel nttpack<:'a> nttunpack<:'a>.
-proof.
-  rewrite /cancel => x.
-  rewrite /nttunpack /nttpack.
-  rewrite -ext_eq_all /all_eq //=.
-qed.
-
-lemma nttunpackK: cancel nttunpack<:'a> nttpack<:'a>.
-proof.
-  rewrite /cancel => x.
-  rewrite /nttunpack /nttpack.
-  rewrite -ext_eq_all /all_eq //=.
-qed.
-
-lemma all_iota P (v : 'a Array256.t) : 
-   Array256.all P v <=> all P (map (fun i => v.[i]) (iotared 0 256)).
-rewrite iotaredE all_map /= /preim /= /#.
-qed.
-
-
 op nttunpackv(v : 'a Array1024.t) = 
    Array1024.init (fun i =>
       if 0 <= i < 256 
@@ -149,12 +85,6 @@ op nttpackv(v : 'a Array1024.t) =
                 then (nttpack (subarray256 v 2)).[i-512]
                 else (nttpack (subarray256 v 3)).[i-768]).
 
-lemma nttpack_bnd : 
-  all (fun x => 0 <= x < 256) nttpack_idx by rewrite all_iota /=.
-
-lemma nttunpack_bnd : 
-  all (fun x => 0 <= x < 256) nttunpack_idx by rewrite all_iota /=.
-
 op nttunpackm(v : 'a Array4096.t) = 
    Array4096.init (fun i =>
       if 0 <= i < 1024 
@@ -174,22 +104,6 @@ op nttpackm(v : 'a Array4096.t) =
            else if 2*1024 <= i < 3*1024
                 then (nttpackv (subarray1024 v 2)).[i-2*1024]
                 else (nttpackv (subarray1024 v 3)).[i-4*1024]).
-
-lemma nttpack_pred (v : 'a Array256.t) P: 
-   (all P (nttpack v)) <=>
-   (all P v).
-rewrite /nttpack /=; split.
-+ rewrite all_iota /=;smt(Array256.initiE Array256.allP).
-rewrite allP all_iota /= /#.
-qed.
-
-lemma nttunpack_pred (v : 'a Array256.t) P: 
-   (all P (nttunpack v)) <=>
-   (all P v).
-rewrite /nttunpack /=; split.
-+ rewrite all_iota /=;smt(Array256.initiE Array256.allP).
-rewrite allP all_iota /= /#.
-qed.
 
 lemma nttpackv_sub (v : 'a Array1024.t) P :
    (all P (nttpack (subarray256 v 0)) /\
@@ -478,209 +392,6 @@ rewrite /unpack. smt(Array1024.initiE Array256.initiE Array256.allP nttunpack_bn
 qed.
 
 
-lemma map_pack (p : 'a Array256.t) (f : 'a -> 'b) : nttpack (Array256.map f p) = map f (nttpack p).
-rewrite /nttpack !mapE.
-rewrite tP => k kb; rewrite !initiE //=.
-pose a:= nttpack_idx.[k].
-rewrite !initiE //=. smt(nttpack_bnd Array256.allP).
-qed.
-
-lemma map_unpack (p : 'a Array256.t) (f : 'a -> 'b) : nttunpack (Array256.map f p) = map f (nttunpack p).
-rewrite /nttunpack !mapE.
-rewrite tP => k kb; rewrite !initiE //=.
-pose a:= nttunpack_idx.[k].
-rewrite !initiE //=. smt(nttunpack_bnd Array256.allP).
-qed.
-
-lemma pack_ext_eq (p q : 'a Array256.t):
-     nttpack p = nttpack q <=> p = q.
-rewrite /nttpack; split;rewrite tP.
-+ move => H. rewrite tP => k kb. 
-  move : (H (nttunpack_idx.[k]) _).  smt(nttunpack_bnd Array256.allP).
-  pose a:= nttunpack_idx.[k].
-  rewrite !initiE //=; 1,2: smt(nttunpack_bnd Array256.allP).
-  rewrite /a. move :nttpack_idxK. rewrite allP; smt( mem_iota).
-move => H. rewrite tP => k kb. 
-  move : (H (nttunpack_idx.[k]) _).  smt(nttunpack_bnd Array256.allP).
-  rewrite !initiE //=; 1: smt(nttpack_bnd Array256.allP).
-qed.
-
-lemma unpack_ext_eq (p q : 'a Array256.t) :
-     nttunpack p = nttunpack q <=> p = q.
-rewrite /nttpack; split;rewrite tP.
-+ move => H. rewrite tP => k kb. 
-  move : (H (nttpack_idx.[k]) _).  smt(nttpack_bnd Array256.allP).
-  pose a:= nttpack_idx.[k].
-  rewrite /nttunpack !initiE //=; 1,2: smt(nttpack_bnd Array256.allP).
-  rewrite /a. move :nttunpack_idxK. rewrite allP; smt( mem_iota).
-move => H. rewrite tP => k kb. 
-  move : (H (nttpack_idx.[k]) _).  smt(nttpack_bnd Array256.allP).
-  rewrite /nttunpack !initiE //=; 1: smt(nttunpack_bnd Array256.allP).
-qed.
-
-lemma pack_bounds (p : W16.t Array256.t) l h:
-     (forall i, 0 <= i < 256 => l <= to_sint p.[i] < h) => (forall i, 0<=i<256 => l <= to_sint (nttpack p).[i] < h).
-move => Hi k.
-move : (nttpack_pred p (fun x => l <= W16.to_sint x < h)); rewrite !allP /= => H.
-move : H => [H1 H2]. 
-move : (H2 Hi). smt().
-qed.
-
-(* FIXME: MERGE W/ pack_bounds *)
-lemma pack_boundsi (p : ipoly) l h:
-     (forall i, 0 <= i < 256 => l <= p.[i] < h) => (forall i, 0 <= i < 256 => l <= (nttpack p).[i] < h).
-proof.
-  move => Hi k.
-  move : (nttpack_pred p (fun x => l <= x < h)); rewrite !allP /= => H.
-  move : H => [H1 H2].
-  move : (H2 Hi). smt().
-qed.
-
-lemma unpack_bounds (p : W16.t Array256.t) l h:
-     (forall i, 0 <= i < 256 => l <= to_sint p.[i] < h) => (forall i, 0<=i<256 => l <= to_sint (nttunpack p).[i] < h).
-proof.
-  move => Hi k.
-  move : (nttunpack_pred p (fun x => l <= W16.to_sint x < h)); rewrite !allP /= => H.
-  move : H => [H1 H2].
-  move : (H2 Hi). smt().
-qed.
-
-(* FIXME: MERGE W/ unpack_bounds *)
-lemma unpack_boundsi (p : ipoly) l h:
-     (forall i, 0 <= i < 256 => l <= p.[i] < h) => (forall i, 0 <= i < 256 => l <= (nttunpack p).[i] < h).
-proof.
-  move => Hi k.
-  move : (nttunpack_pred p (fun x => l <= x < h)); rewrite !allP /= => H.
-  move : H => [H1 H2].
-  move : (H2 Hi). smt().
-qed.
-
-
-lemma pack128_bounds (p: W16.t Array256.t) k l h:
-      0 <= k < 3 => (forall i, 0 <= i < 128 * k => l <= to_sint p.[i] < h) => (forall i, 0 <= i < 128 * k => l <= to_sint (nttpack p).[i] < h).
-proof.
-  rewrite andabP => /(mem_iota 0 3 k).
-  move : k.
-  rewrite -(List.allP (fun x => (forall (i : int), 0 <= i && i < 128 * x => l <= to_sint p.[i] && to_sint p.[i] < h) =>
-                                (forall (i : int), 0 <= i && i < 128 * x => l <= to_sint (nttpack p).[i] && to_sint (nttpack p).[i] < h))).
-  rewrite -iotaredE //=.
-  do split; first by smt(@Logic).
-    + move => Hi i.
-      rewrite andabP => /(mem_iota 0 128 i).
-      move : i.
-      rewrite -(List.allP (fun i => l <= to_sint (nttpack p).[i] && to_sint (nttpack p).[i] < h)).
-      rewrite -iotaredE //=.
-      rewrite /nttpack initiE 1://= //=.
-      by do (rewrite Hi 1://=).
-    + apply pack_bounds.
-qed.
-
-lemma unpack128_bounds (p: W16.t Array256.t) k l h:
-      0 <= k < 3 => (forall i, 0 <= i < 128 * k => l <= to_sint p.[i] < h) => (forall i, 0 <= i < 128 * k => l <= to_sint (nttunpack p).[i] < h).
-proof.
-  rewrite andabP => /(mem_iota 0 3 k).
-  move : k.
-  rewrite -(List.allP (fun x => (forall (i : int), 0 <= i && i < 128 * x => l <= to_sint p.[i] && to_sint p.[i] < h) =>
-                                (forall (i : int), 0 <= i && i < 128 * x => l <= to_sint (nttunpack p).[i] && to_sint (nttunpack p).[i] < h))).
-  rewrite -iotaredE //=.
-  do split; first by smt(@Logic).
-    + move => Hi i.
-      rewrite andabP => /(mem_iota 0 128 i).
-      move : i.
-      rewrite -(List.allP (fun i => l <= to_sint (nttunpack p).[i] && to_sint (nttunpack p).[i] < h)).
-      rewrite -iotaredE //=.
-      rewrite /nttunpack initiE 1://= //=.
-      by do (rewrite Hi 1://=).
-    + apply unpack_bounds.
-qed.
-
-lemma pack128_boundsi (p: ipoly) k l h:
-      0 <= k < 3 => (forall i, 0 <= i < 128 * k => l <= p.[i] < h) => (forall i, 0 <= i < 128 * k => l <= (nttpack p).[i] < h).
-proof.
-  rewrite andabP => /(mem_iota 0 3 k).
-  move : k.
-  rewrite -(List.allP (fun x => (forall (i : int), 0 <= i && i < 128 * x => l <= p.[i] && p.[i] < h) =>
-                                (forall (i : int), 0 <= i && i < 128 * x => l <= (nttpack p).[i] && (nttpack p).[i] < h))).
-  rewrite -iotaredE //=.
-  do split; first by smt(@Logic).
-    + move => Hi i.
-      rewrite andabP => /(mem_iota 0 128 i).
-      move : i.
-      rewrite -(List.allP (fun i => l <= (nttpack p).[i] && (nttpack p).[i] < h)).
-      rewrite -iotaredE //=.
-      rewrite /nttpack initiE 1://= //=.
-      by do (rewrite Hi 1://=).
-    + apply pack_boundsi.
-qed.
-
-
-lemma unpack128_boundsi (p: ipoly) k l h:
-      0 <= k < 3 => (forall i, 0 <= i < 128 * k => l <= p.[i] < h) => (forall i, 0 <= i < 128 * k => l <= (nttunpack p).[i] < h).
-proof.
-  rewrite andabP => /(mem_iota 0 3 k).
-  move : k.
-  rewrite -(List.allP (fun x => (forall (i : int), 0 <= i && i < 128 * x => l <= p.[i] && p.[i] < h) =>
-                                (forall (i : int), 0 <= i && i < 128 * x => l <= (nttunpack p).[i] && (nttunpack p).[i] < h))).
-  rewrite -iotaredE //=.
-  do split; first by smt(@Logic).
-    + move => Hi i.
-      rewrite andabP => /(mem_iota 0 128 i).
-      move : i.
-      rewrite -(List.allP (fun i => l <= (nttunpack p).[i] && (nttunpack p).[i] < h)).
-      rewrite -iotaredE //=.
-      rewrite /nttunpack initiE 1://= //=.
-      by do (rewrite Hi 1://=).
-    + apply unpack_boundsi.
-qed.
-
-lemma nttpack_inbounds: forall k, 0 <= k < 256 => 0 <= nttpack_idx.[k] && nttpack_idx.[k] < 256.
-proof.
-  apply (Array256.allP _ (fun x => 0 <= x && x < 256)).
-  rewrite /Array256.all -iotaredE //=.
-qed.
-
-lemma nttunpack_inbounds: forall k, 0 <= k < 256 => 0 <= nttunpack_idx.[k] && nttunpack_idx.[k] < 256.
-proof.
-  apply (Array256.allP _ (fun x => 0 <= x && x < 256)).
-  rewrite /Array256.all -iotaredE //=.
-qed.
-
-lemma nttpack128_bounds: forall k, 0 <= k < 256 => (k %/ 128) * 128 <= nttpack_idx.[k] && nttpack_idx.[k] < (k %/ 128) * 128 + 128.
-proof.
-  move => k.
-  rewrite andabP => /(mem_iota 0 256 k).
-  move : k.
-  rewrite -(List.allP (fun x => (x %/ 128) * 128 <= nttpack_idx.[x] && nttpack_idx.[x] < (x %/ 128) * 128 + 128) _).
-  rewrite -iotaredE //=.
-qed.
-
-lemma nttunpack128_bounds: forall k, 0 <= k < 256 => (k %/ 128) * 128 <= nttunpack_idx.[k] && nttunpack_idx.[k] < (k %/ 128) * 128 + 128.
-proof.
-  move => k.
-  rewrite andabP => /(mem_iota 0 256 k).
-  move : k.
-  rewrite -(List.allP (fun x => (x %/ 128) * 128 <= nttunpack_idx.[x] && nttunpack_idx.[x] < (x %/ 128) * 128 + 128) _).
-  rewrite -iotaredE //=.
-qed.
-
-lemma lift_nttpack v : lift_array256 (nttpack v) = nttpack (lift_array256 v).
-proof. 
-rewrite tP => k kb.
-rewrite /lift_array256 mapiE //=.
-rewrite /nttpack !initiE //=.
-pose a := nttpack_idx.[k].
-smt(Array256.mapiE nttpack_bnd Array256.allP).
-qed.
-
-lemma lift_nttunpack v : lift_array256 (nttunpack v) = nttunpack (lift_array256 v).
-proof. 
-rewrite tP => k kb.
-rewrite /lift_array256 mapiE //=.
-rewrite /nttunpack !initiE //=.
-pose a := nttunpack_idx.[k].
-smt(Array256.mapiE nttunpack_bnd Array256.allP).
-qed.
-
 lemma init_unpack (v : 'a Array1024.t) :
   Array256.init ("_.[_]" (nttunpackv v)) = nttunpack (Array256.init ("_.[_]" v)).
 rewrite /nttunpackv /nttunpack tP => k kb.
@@ -736,53 +447,7 @@ rewrite -/a initiE //=.
  smt(nttunpack_bnd Array256.allP).
 qed.
 
-lemma lift256_nttunpack v :
-  lift_array256 (nttunpack v) = nttunpack (lift_array256 v).
-rewrite /lift_array256 /nttunpack tP => k kb.
-rewrite mapiE //= initiE //=.
-pose a:= nttunpack_idx.[k].
-rewrite initiE //= mapiE //=. smt(nttunpack_bnd Array256.allP).
-qed.
-
-from JazzEC require import Jkem_avx2.
 require import NTT_AVX_Fq NTT_AVX_j.
-
-lemma perm_ntt_nttpackE ['a] (p: 'a Array256.t):
-  perm_ntt NTT_AVX_Fq.perm_nttpack128 p = nttpack p.
-proof.
-by apply Array256.all_eq_eq; rewrite /all_eq 
-   /perm_ntt /perm_nttpack128 /nttpack /=.
-qed.
-
-phoare poly_basemul_avx2_ph _a _b:
- [Jkem_avx2.M._poly_basemul:
-    (lift_array256 ap) = nttunpack _a /\ signed_bound_cxq ap 0 256 2
-    /\ (lift_array256 bp) = nttunpack _b /\ signed_bound_cxq bp 0 256 2
-   ==>
-    (lift_array256 res)
-    = nttunpack (scale (basemul (_a) (_b)) (incoeff 169))
-    /\ signed_bound_cxq res 0 256 1 ] = 1%r.
-proof. 
-conseq poly_basemul_avx2_eq (__basemul_ph (nttunpack _a) (nttunpack _b)) => //.
- move => /> &1 *.
- by exists ((lift_array256 rp{1}), (lift_array256 ap{1}), (lift_array256 bp{1})) => //=.
-move=> /> &m <- Hb.
-move: (basemul_avx2E (nttunpack _a) (nttunpack _b)).
-rewrite !perm_ntt_nttpackE !nttunpackK => <-.
-by rewrite /scale -map_pack nttpackK.
-qed.
-
-lemma poly_ntt_avx2_corr _r :
-  phoare [Jkem_avx2.M._poly_ntt :
-    rp = _r /\ signed_bound_cxq rp 0 256 2 ==>
-    ntt (lift_array256 _r) = lift_array256 (nttpack res) /\
-    pos_bound256_cxq res 0 256 2] = 1%r.
-proof.
-conseq poly_ntt_avx2_eq (ntt_avx_spec (lift_array256 _r)).
- by move => &1 [-> H] /#.
-move=> &1 &2 [-> H] <-.
-by rewrite lift_nttpack perm_ntt_nttpackE.
-qed.
 
 import KMatrix.
 import Vector.
@@ -808,8 +473,8 @@ move => [#] H7 H8 r1 H9 H10. do split.
 + rewrite tP => k kb; rewrite !initiE //= initiE //= 1: /# ifF 1:/# initiE //= 1:/# ifF 1:/# initiE //= /#.
 + rewrite /signed_bound_cxq => k kb; rewrite !initiE //= initiE //= 1: /# ifF 1:/# initiE //= 1:/# ifF 1:/# initiE //= /#.
 move => [#] H11 HH12 r2 H13 H14. do split.
-+ rewrite /nttv /lift_polyvec eq_vectorP => k kb.
-  rewrite mapvE !offunvE //= KMatrix.Vector.offunvK /vclamp kb /=.
++ apply KVec.tP => k kb. have kv := kvec_val.
+  rewrite /nttv /mapv KVec.mapiE 1:/# /lift_polyvec !KVec.initiE 1,2:/# /=.
   rewrite /lift_array256 /subarray256 tP => i ib.
   rewrite mapiE //= initiE //= /nttpackv initiE //= 1:/#.
   move :nttunpack_bnd nttpack_bnd; rewrite !allP => pb upb.
@@ -848,17 +513,6 @@ rewrite /pos_bound1024_cxq => k kb; rewrite initiE //=.
  move => *;case(256 <= k < 512). 
   + move => *; rewrite initiE //=  initiE //=. smt(). 
   move => *; rewrite initiE //= ifF 1:/# initiE //= initiE //= /#. 
-qed.
-
-lemma poly_invntt_avx2_corr _r :
-  phoare [Jkem_avx2.M._poly_invntt :
-    lift_array256 (nttpack rp) = lift_array256 _r /\ signed_bound_cxq rp 0 256 4 ==>
-    mul1x256 (incoeff W16.modulus) (invntt (lift_array256 _r)) = (lift_array256 res) /\
-    signed_bound_cxq res 0 256 1] = 1%r.
-proof.
-conseq poly_invntt_avx2_eq (invntt_avx_spec (lift_array256 _r)).
-move => &1 [<- H]. exists (lift_array256 arg{1}) => />. rewrite lift_nttpack perm_ntt_nttpackE //.
-move => &1 &2 [<- H] -> /#. 
 qed.
 
 lemma nttpack_subarray1024 (r : 'a Array1024.t) :
@@ -936,36 +590,43 @@ do split.
  + by rewrite /signed_bound_cxq => i Hi; rewrite !initiE 1:/# /= !initiE 1:/# /=  !initiE 1:/# /= !initiE 1:/# /=/#.
 
 move => r2 [#] Hr2 H10.  
-do split. 
- + rewrite /lift_polyvec eq_vectorP => k Hk; rewrite !offunvE //=.
-   rewrite /lift_array256 /subarray256 tP => i Hi.
-   rewrite !mapiE //= initiE //= /nttpackv initiE //= 1:/# /nttv /invnttv. 
- + case (k=0).
-  + move => ->; rewrite ifF 1:/# initiE //= 1:/# ifF 1:/# initiE //= 1:/# ifF 1:/# // initiE 1:/# /= ifT 1:/# //.
-    move :Hr; rewrite /lift_array256 tP => /> Hr.  move :(Hr i); rewrite Hi /map !initiE //=. move => H12. 
-    rewrite !mapvE /= !offunvE /= 1:/# initiE 1:/# /=.
-    rewrite !offunvK /vclamp !ifT 1,2:/# /= /#.
- + case (k=1).
-  + move => -> ?. rewrite ifF 1:/# initiE //= 1:/# ifF 1:/#.  
-  + move :Hr0. rewrite !mapvE /lift_array256 tP => /> Hr0. move :(Hr0 i). 
-    rewrite Hi /map !initiE //= 1:/# ifT 1:/# !offunvK /vclamp /= !offunvE /= 1:/# initiE /#.  
- + case (k=2).
-  + move => -> ? ?. rewrite ifF 1:/# initiE //= 1:/# ifT 1:/# /=.  
-  + move :Hr1. rewrite !mapvE /lift_array256 tP => /> Hr1. move :(Hr1 i). 
-    rewrite Hi /map !initiE //=. rewrite !offunvK /vclamp /= !offunvE /= 1:/# initiE /#.  
- + move => *; have -> : k = 3 by smt().
-  + rewrite ifT 1:/#.
-  + move :Hr2. rewrite !mapvE /lift_array256 tP => /> Hr2. 
-    move :(Hr2 i). rewrite Hi /map !initiE //=.
-    rewrite !offunvK /vclamp /= !offunvE /= 1:/# initiE /#. 
-  + rewrite /signed_bound1024_cxq => k Hk; rewrite initiE /= 1:/#.
- + case(768 <= k < 1024). smt().
- + move => *;case(512 <= k < 768). 
- + move => *; rewrite initiE /= /#.
- + move => *;case(256 <= k < 512). 
- + move => *; rewrite initiE 1:/# /= initiE /#.
- + move => *; rewrite initiE 1:/# /=  ifF 1:/# initiE //= initiE //= /#. 
+split.
+ + apply KVec.tP => k Hk.
+   rewrite /mul1x256v /mapv KVec.mapiE 1:/# invnttvE 1:/# /lift_polyvec !KVec.initiE 1,2:/#.
+   simplify.
+   case (k=0) => [->|hkn0].
+   + have e1: subarray256 _r 0 = init (fun (i0:int) => _r.[i0]).
+     + apply Array256.tP => j hj; rewrite /subarray256 !initiE 1,2:/#; smt().
+     rewrite e1 Hr; congr.
+     apply Array256.tP => j hj; rewrite /subarray256 Array256.initiE 1:/# /=; smt(Array1024.initiE).
+   case (k=1) => [->|hkn1].
+   + have e2: subarray256 _r 1 = init (fun (i0:int) => _r.[256+i0]).
+     + apply Array256.tP => j hj; rewrite /subarray256 !initiE 1,2:/#; smt().
+     rewrite e2 Hr0; congr.
+     apply Array256.tP => j hj; rewrite /subarray256 Array256.initiE 1:/# /=; smt(Array1024.initiE).
+   case (k=2) => [->|hkn2].
+   + have e3: subarray256 _r 2 = init (fun (i0:int) => _r.[512+i0]).
+     + apply Array256.tP => j hj; rewrite /subarray256 !initiE 1,2:/#; smt().
+     rewrite e3 Hr1; congr.
+     apply Array256.tP => j hj; rewrite /subarray256 Array256.initiE 1:/# /=; smt(Array1024.initiE).
+   have kv := kvec_val.
+   have ->: k = 3 by smt().
+   have e4: subarray256 _r 3 = init (fun (i0:int) => _r.[768+i0]).
+   + apply Array256.tP => j hj; rewrite /subarray256 !initiE 1,2:/#; smt().
+   rewrite e4 Hr2; congr.
+   apply Array256.tP => j hj; rewrite /subarray256 Array256.initiE 1:/# /=; smt(Array1024.initiE).
+ + rewrite /signed_bound1024_cxq => i Hi; rewrite Array1024.initiE 1:/# /=.
+   case (768 <= i < 1024) => hi1.
+   + move: H10; rewrite /signed_bound_cxq => H10; smt().
+   rewrite Array1024.initiE 1:/# /=.
+   case (512 <= i < 768) => hi2.
+   + move: H8; rewrite /signed_bound_cxq => H8; smt().
+   rewrite Array1024.initiE 1:/# /=.
+   case (256 <= i < 512) => hi3.
+   + move: H7; rewrite /signed_bound_cxq => H7; smt().
+   rewrite Array1024.initiE 1:/# /=.
+   move: H4; rewrite /signed_bound_cxq => H4; smt().
 qed.
 
+
 end NTT_Avx2.
- 
