proof/correctness/avx2/common/MLKEM_Poly_avx2.ec
@@ -1,0 +1,1854 @@
+(* ==== from.ec ==== *)
+require import AllCore List Int IntDiv CoreMap Real Number.
+
+from Jasmin require import JModel JMemory JWord.
+from JazzEC require import Array400 Array256 Array128 Array64 Array32 Array16 Array8 Array4 Array2.
+from JazzEC require import WArray800 WArray512 WArray128 WArray128 WArray64 WArray32 WArray16.
+from JazzEC require import Jkem_avx2.
+
+require import AVX2_Ops.
+
+require import MLKEM_avx2_auxlemmas.
+
+module Mprevec = {
+  proc shuffle8 (a:t16u16, b:t16u16) : t16u16 * t16u16 = {
+    
+    var r0:t16u16;
+    var r1:t16u16;
+    
+    r0 <@ Ops.iVPERM2I128_16u16(a, b, (W8.of_int 32));
+    r1 <@ Ops.iVPERM2I128_16u16(a, b, (W8.of_int 49));
+
+    return (r0, r1);
+  }
+  
+  proc shuffle4 (a:t16u16, b:t16u16) : t16u16 * t16u16 = {
+    
+    var r0:t16u16;
+    var r1:t16u16;
+    
+    r0 <@ Ops.iVPUNPCKL_4u64_16u16(a, b);
+    r1 <@ Ops.iVPUNPCKH_4u64_16u16(a, b);
+
+    return (r0, r1);
+  }
+  
+  proc shuffle2 (a:t16u16, b:t16u16) : t16u16 * t16u16 = {
+    
+    var t0:t16u16;
+    var t1:t16u16;
+    var a_q: t4u64;
+    
+    t0  <@ Ops.iVMOVSLDUP_256_16u16(b);
+    t0  <@ Ops.iVPBLEND_8u32_16u16(a, t0, (W8.of_int 170));
+    a_q <- f16u16_t4u64 a;
+    a_q <@ Ops.iVPSRL_4u64(a_q, (W8.of_int 32));
+    a <- f4u64_t16u16 a_q;
+    t1 <@ Ops.iVPBLEND_8u32_16u16(a, b, (W8.of_int 170));
+    return (t0, t1);
+  }
+  
+  proc shuffle1 (a:t16u16, b:t16u16) : t16u16 * t16u16 = {
+    
+    var r0:t16u16;
+    var r1:t16u16;
+    var t0:t16u16;
+    var t1:t16u16;
+    var t0_d:t8u32;
+    var t1_d:t8u32;
+    var a_d:t8u32;
+    var b_d:t8u32;
+
+    b_d <- f16u16_t8u32 b;
+    t0_d <@ Ops.iVPSLL_8u32(b_d, (W8.of_int 16));
+    t0 <- f8u32_t16u16 t0_d;
+    r0 <@ Ops.iVPBLEND_16u16(a, t0, (W8.of_int 170));
+    a_d <- f16u16_t8u32 a;
+    t1_d <@ Ops.iVPSRL_8u32(a_d, (W8.of_int 16));
+    t1 <- f8u32_t16u16 t1_d;
+    r1 <@ Ops.iVPBLEND_16u16(t1, b, (W8.of_int 170));
+
+    return (r0, r1);
+  }
+
+  proc poly_add2(rp:W16.t Array256.t, bp:W16.t Array256.t) : W16.t Array256.t = {
+    var i:int;
+    var a:W16.t Array16.t;
+    var b:W16.t Array16.t;
+    var r:W16.t Array16.t;
+
+    i <- 0;
+
+    while (i < 16) {
+      a <- lift2poly(get256_direct (WArray512.init16 (fun i => rp.[i])) (32 * i));
+      b <- lift2poly(get256_direct (WArray512.init16 (fun i => bp.[i])) (32 * i));
+
+      r <@ Ops.iVPADD_16u16(a, b);
+
+      rp <- fill (fun k => r.[k %% 16]) (16*i) 16 rp;
+
+      i <- i + 1;
+    }
+
+    return rp;
+  }
+
+  proc poly_sub(rp:W16.t Array256.t, ap:W16.t Array256.t,
+                 bp:W16.t Array256.t) : W16.t Array256.t = {
+    var aux: int;
+
+    var i:int;
+    var a:W16.t Array16.t;
+    var b:W16.t Array16.t;
+    var r:W16.t Array16.t;
+
+    i <- 0;
+    while (i < 16) {
+      a <- lift2poly(get256_direct (WArray512.init16 (fun i => ap.[i])) (32 * i));
+      b <- lift2poly(get256_direct (WArray512.init16 (fun i => bp.[i])) (32 * i));
+
+      r <@ Ops.iVPSUB_16u16(a, b);
+
+      rp <- fill (fun k => r.[k %% 16]) (16*i) 16 rp;
+
+      i <- i + 1;
+    }
+
+    return (rp);
+  }
+
+  proc csubq (r:t16u16, qx16:t16u16) : t16u16 = {
+    var t:t16u16;
+
+    r <@ Ops.iVPSUB_16u16(r, qx16);
+    t <@ Ops.iVPSRA_16u16(r, (W8.of_int 15));
+    t <@ Ops.iVPAND_16u16(t,qx16);
+    r <@ Ops.iVPADD_16u16(t, r);
+
+    return r;
+  }
+
+  proc poly_csubq (rp:W16.t Array256.t) : W16.t Array256.t = {
+    var aux: int;
+
+    var qx16:W256.t;
+    var _qx16: W16.t Array16.t;
+    var i:int;
+    var r:W256.t;
+    var _r: W16.t Array16.t;
+    var t: W16.t Array16.t;
+
+    qx16 <- (get256 (WArray32.init16 (fun i => jqx16.[i])) 0);
+    _qx16 <- lift2poly(qx16);
+    i <- 0;
+    while (i < 16) {
+      r <- (get256_direct (WArray512.init16 (fun i => rp.[i])) (32 * i));
+
+      _r <- lift2poly(r);
+
+      _r <@ Ops.iVPSUB_16u16(_r, _qx16);
+      t <@ Ops.iVPSRA_16u16(_r, (W8.of_int 15));
+      t <@ Ops.iVPAND_16u16(t, _qx16);
+      _r <@ Ops.iVPADD_16u16(t, _r);
+
+      rp <- fill (fun k => _r.[k %% 16]) (16*i) 16 rp;
+
+      i <- i + 1;
+    }
+    return (rp);
+  }
+
+  proc fqmulx16 (a b qx16 qinvx16: W16.t Array16.t) : W16.t Array16.t = {
+
+    var rd:W16.t Array16.t;
+    var rhi:W16.t Array16.t;
+    var rlo:W16.t Array16.t;
+
+    rhi <@ Ops.iVPMULH_256(a, b);
+    rlo <@ Ops.iVPMULL_16u16(a, b);
+    rlo <@ Ops.iVPMULL_16u16(rlo, qinvx16);
+    rlo <@ Ops.iVPMULH_256(rlo, qx16);
+    rd <@  Ops.iVPSUB_16u16(rhi, rlo);
+    return (rd);
+  }
+
+
+  (*--------------------------------------------------------------------*)
+
+  proc red16x (r:W16.t Array16.t, qx16:W16.t Array16.t, vx16:W16.t Array16.t) : W16.t Array16.t = {
+    var x:W16.t Array16.t;
+
+    x <@ Ops.iVPMULH_256(r, vx16);
+    x <@ Ops.iVPSRA_16u16(x, (W8.of_int 10));
+    x <@ Ops.iVPMULL_16u16(x, qx16);
+    r <@ Ops.iVPSUB_16u16(r, x);
+
+    return (r);
+  }
+
+  proc poly_reduce (rp:W16.t Array256.t) : W16.t Array256.t = {
+    var aux: int;
+
+    var qx16:W16.t Array16.t;
+    var vx16:W16.t Array16.t;
+    var i:int;
+    var r:W16.t Array16.t;
+
+    qx16 <- lift2poly (get256 (WArray32.init16 (fun i => jqx16.[i])) 0);
+    vx16 <- lift2poly (get256 (WArray32.init16 (fun i => jvx16.[i])) 0);
+    i <- 0;
+
+    while (i < 16) {
+      r <- lift2poly (get256_direct (WArray512.init16 (fun i => rp.[i])) (32 * i));
+
+      r <@ red16x (r, qx16, vx16);
+
+      rp <- fill (fun k => r.[k %% 16]) (16*i) 16 rp;
+
+      i <- i + 1;
+    }
+    return (rp);
+  }
+
+  proc poly_frommont (rp:W16.t Array256.t) : W16.t Array256.t = {
+    var aux: int;
+
+    var qx16:W16.t Array16.t;
+    var qinvx16:W16.t Array16.t;
+    var dmontx16:W16.t Array16.t;
+    var i:int;
+    var t:W16.t Array16.t;
+
+    qx16 <- lift2poly(get256 (WArray32.init16 (fun i => jqx16.[i])) 0);
+    qinvx16 <- lift2poly(get256 (WArray32.init16 (fun i => jqinvx16.[i])) 0);
+    dmontx16 <- lift2poly(get256 (WArray32.init16 (fun i => jdmontx16.[i])) 0);
+    aux <- (256 %/ 16);
+
+    i <- 0;
+    while (i < aux) {
+      t <- lift2poly(get256 (WArray512.init16 (fun i => rp.[i])) i);
+      t <@ fqmulx16 (t, dmontx16, qx16, qinvx16);
+
+      rp <- fill (fun k => t.[k %% 16]) (16*i) 16 rp;
+
+      i <- i + 1;
+    }
+    return (rp);
+  }
+
+  proc schoolbook (ap:W16.t Array32.t, bp:W16.t Array32.t, zeta_0: t16u16,
+                   qx16:t16u16, qinvx16:t16u16, sign:int) : t16u16 * t16u16 *
+                                                            t16u16 * t16u16 = {
+
+    var x0:t16u16;
+    var x1:t16u16;
+    var y0:t16u16;
+    var y1:t16u16;
+    var b:t16u16;
+    var d:t16u16;
+    var a:t16u16;
+    var c:t16u16;
+    var bdlo:t16u16;
+    var bdhi:t16u16;
+    var bclo:t16u16;
+    var bchi:t16u16;
+    var adlo:t16u16;
+    var adhi:t16u16;
+    var aclo:t16u16;
+    var achi:t16u16;
+    var bd:t16u16;
+    var rbdlo:t16u16;
+    var rbdhi:t16u16;
+    var bc0:t16u16;
+    var bc1:t16u16;
+    var ad0:t16u16;
+    var ad1:t16u16;
+    var ac0:t16u16;
+    var ac1:t16u16;
+    var rbd0:t16u16;
+    var rbd1:t16u16;
+
+    var x0_dw:t8u32;
+    var x1_dw:t8u32;
+    var y0_dw:t8u32;
+    var y1_dw:t8u32;
+    var bc0_dw:t8u32;
+    var bc1_dw:t8u32;
+    var ad0_dw:t8u32;
+    var ad1_dw:t8u32;
+    var ac0_dw: t8u32;
+    var ac1_dw: t8u32;
+    var rbd0_dw: t8u32;
+    var rbd1_dw: t8u32;
+
+
+    b <- Array16.init (fun i => ap.[16 + i]);
+    d <- Array16.init (fun i => bp.[16 + i]);
+    a <- Array16.init (fun i => ap.[i]);
+    c <- Array16.init (fun i => bp.[i]);
+    bdlo <@ Ops.iVPMULL_16u16(b, d);
+    bdhi <@ Ops.iVPMULH_256(b, d);
+    bclo <@ Ops.iVPMULL_16u16(b, c);
+    bchi <@ Ops.iVPMULH_256(b, c);
+    adlo <@ Ops.iVPMULL_16u16(a, d);
+    adhi <@ Ops.iVPMULH_256(a, d);
+    aclo <@ Ops.iVPMULL_16u16(a, c);
+    achi <@ Ops.iVPMULH_256(a, c);
+    bdlo <@ Ops.iVPMULL_16u16(bdlo, qinvx16);
+    bdlo <@ Ops.iVPMULH_256(bdlo, qx16);
+    bd <@ Ops.iVPSUB_16u16(bdhi, bdlo);
+    rbdlo <@ Ops.iVPMULL_16u16(zeta_0, bd);
+    rbdhi <@ Ops.iVPMULH_256(zeta_0, bd);
+    bc0 <@ Ops.iVPUNPCKL_16u16(bclo, bchi);
+    bc1 <@ Ops.iVPUNPCKH_16u16(bclo, bchi);
+    ad0 <@ Ops.iVPUNPCKL_16u16(adlo, adhi);
+    ad1 <@ Ops.iVPUNPCKH_16u16(adlo, adhi);
+    ac0 <@ Ops.iVPUNPCKL_16u16(aclo, achi);
+    ac1 <@ Ops.iVPUNPCKH_16u16(aclo, achi);
+    rbd0 <@ Ops.iVPUNPCKL_16u16(rbdlo, rbdhi);
+    rbd1 <@ Ops.iVPUNPCKH_16u16(rbdlo, rbdhi);
+
+    ac0_dw <- f16u16_t8u32 ac0;
+    rbd0_dw <- f16u16_t8u32 rbd0;
+
+    ac1_dw <- f16u16_t8u32 ac1;
+    rbd1_dw <- f16u16_t8u32 rbd1;
+
+    bc0_dw <- f16u16_t8u32 bc0;
+    bc1_dw <- f16u16_t8u32 bc1;
+    ad0_dw <- f16u16_t8u32 ad0;
+    ad1_dw <- f16u16_t8u32 ad1;
+
+    if ((sign = 0)) {
+      x0_dw <@ Ops.iVPADD_8u32(ac0_dw, rbd0_dw);
+      x1_dw <@ Ops.iVPADD_8u32(ac1_dw, rbd1_dw);
+    } else {
+      x0_dw <@ Ops.iVPSUB_8u32(ac0_dw, rbd0_dw);
+      x1_dw <@ Ops.iVPSUB_8u32(ac1_dw, rbd1_dw);
+    }
+    y0_dw <@ Ops.iVPADD_8u32(bc0_dw, ad0_dw);
+    y1_dw <@ Ops.iVPADD_8u32(bc1_dw, ad1_dw);
+
+    x0 <- f8u32_t16u16 x0_dw;
+    x1 <- f8u32_t16u16 x1_dw;
+    y0 <- f8u32_t16u16 y0_dw;
+    y1 <- f8u32_t16u16 y1_dw;
+
+    return (x0, x1, y0, y1);
+  }
+
+  proc basemul_red (a0:t16u16, a1:t16u16, b0:t16u16, b1:t16u16, qx16:t16u16,
+                    qinvx16:t16u16) : t16u16 * t16u16 = {
+
+    var zero:t16u16;
+    var y:t16u16;
+    var z:t16u16;
+    var x:t16u16;
+
+    var a0_dw: t8u32;
+    var a1_dw: t8u32;
+    var b0_dw: t8u32;
+    var b1_dw: t8u32;
+    var y_dw: t8u32;
+    var z_dw: t8u32;
+    var x_dw: t8u32;
+
+    zero <- lift2poly(W256.zero);
+    y <@ Ops.iVPBLEND_16u16(a0, zero, (W8.of_int 170));
+    z <@ Ops.iVPBLEND_16u16(a1, zero, (W8.of_int 170));
+
+    a0_dw <- f16u16_t8u32 a0;
+    a1_dw <- f16u16_t8u32 a1;
+    z_dw <- f16u16_t8u32 z;
+    y_dw <- f16u16_t8u32 y;
+
+    a0_dw <@ Ops.iVPSRL_8u32(a0_dw, (W8.of_int 16));
+    a1_dw <@ Ops.iVPSRL_8u32(a1_dw, (W8.of_int 16));
+    z <@ Ops.iVPACKUS_8u32(y_dw, z_dw);
+    a0 <@ Ops.iVPACKUS_8u32(a0_dw, a1_dw);
+
+    y <@ Ops.iVPBLEND_16u16(b0, zero, (W8.of_int 170));
+    x <@ Ops.iVPBLEND_16u16(b1, zero, (W8.of_int 170));
+
+    b0_dw <- f16u16_t8u32 b0;
+    b1_dw <- f16u16_t8u32 b1;
+    x_dw <- f16u16_t8u32 x;
+    y_dw <- f16u16_t8u32 y;
+
+    b0_dw <@ Ops.iVPSRL_8u32(b0_dw, (W8.of_int 16));
+    b1_dw <@ Ops.iVPSRL_8u32(b1_dw, (W8.of_int 16));
+    y <@ Ops.iVPACKUS_8u32(y_dw, x_dw);
+    b0 <@ Ops.iVPACKUS_8u32(b0_dw, b1_dw);
+
+    z <@ Ops.iVPMULL_16u16(z, qinvx16);
+    y <@ Ops.iVPMULL_16u16(y, qinvx16);
+    z <@ Ops.iVPMULH_256(z, qx16);
+    y <@ Ops.iVPMULH_256(y, qx16);
+    a0 <@ Ops.iVPSUB_16u16(a0, z);
+    b0 <@ Ops.iVPSUB_16u16(b0, y);
+    return (a0, b0);
+  }
+
+  proc basemul32x (rp:W16.t Array64.t, ap:W16.t Array64.t,
+                   bp:W16.t Array64.t, zeta_0:t16u16, qx16:t16u16,
+                   qinvx16:t16u16) : W16.t Array64.t = {
+
+    var x0:t16u16;
+    var x1:t16u16;
+    var y0:t16u16;
+    var y1:t16u16;
+
+    (x0, x1, y0, y1) <@ schoolbook ((Array32.init (fun i => ap.[0 + i])),
+    (Array32.init (fun i => bp.[0 + i])), zeta_0, qx16, qinvx16, 0);
+    (x0, x1) <@ basemul_red (x0, x1, y0, y1, qx16, qinvx16);
+
+    rp <- fill (fun k => x0.[k %% 16]) 0 16 rp;
+    rp <- fill (fun k => x1.[k %% 16]) 16 16 rp;
+
+    (x0, x1, y0, y1) <@ schoolbook ((Array32.init (fun i => ap.[32 + i])),
+    (Array32.init (fun i => bp.[32 + i])), zeta_0, qx16, qinvx16, 1);
+    (x0, x1) <@ basemul_red (x0, x1, y0, y1, qx16, qinvx16);
+
+    rp <- fill (fun k => x0.[k %% 16]) 32 16 rp;
+    rp <- fill (fun k => x1.[k %% 16]) 48 16 rp;
+
+    return (rp);
+  }
+
+  proc poly_basemul (rp:W16.t Array256.t, ap:W16.t Array256.t,
+                     bp:W16.t Array256.t) : W16.t Array256.t = {
+    var aux: W16.t Array64.t;
+
+    var qx16:t16u16;
+    var qinvx16:t16u16;
+    var zeta_0:t16u16;
+
+    qx16 <- lift2poly(get256_direct (WArray32.init16 (fun i => jqx16.[i])) 0);
+    qinvx16 <- lift2poly(get256_direct (WArray32.init16 (fun i => jqinvx16.[i])) 0);
+    zeta_0 <-
+    lift2poly(get256_direct (WArray800.init16 (fun i => jzetas_exp.[i])) 304);
+
+    aux <@ basemul32x ((Array64.init (fun i => rp.[0 + i])),
+    (Array64.init (fun i => ap.[0 + i])),
+    (Array64.init (fun i => bp.[0 + i])), zeta_0, qx16, qinvx16);
+
+    rp <- fill (fun k => aux.[k %% 64]) 0 64 rp;
+
+    zeta_0 <-
+    lift2poly(get256_direct (WArray800.init16 (fun i => jzetas_exp.[i])) 368);
+
+    aux <@ basemul32x ((Array64.init (fun i => rp.[64 + i])),
+    (Array64.init (fun i => ap.[64 + i])),
+    (Array64.init (fun i => bp.[64 + i])), zeta_0, qx16, qinvx16);
+
+    rp <- fill (fun k => aux.[k %% 64]) 64 64 rp;
+
+    zeta_0 <-
+    lift2poly(get256_direct (WArray800.init16 (fun i => jzetas_exp.[i])) 696);
+
+    aux <@ basemul32x ((Array64.init (fun i => rp.[128 + i])),
+    (Array64.init (fun i => ap.[128 + i])),
+    (Array64.init (fun i => bp.[128 + i])), zeta_0, qx16, qinvx16);
+
+    rp <- fill (fun k => aux.[k %% 64]) 128 64 rp;
+
+    zeta_0 <-
+    lift2poly(get256_direct (WArray800.init16 (fun i => jzetas_exp.[i])) 760);
+
+    aux <@ basemul32x ((Array64.init (fun i => rp.[192 + i])),
+    (Array64.init (fun i => ap.[192 + i])),
+    (Array64.init (fun i => bp.[192 + i])), zeta_0, qx16, qinvx16);
+
+    rp <- fill (fun k => aux.[k %% 64]) 192 64 rp;
+
+    return (rp);
+  }
+
+}.
+
+(* ==== from.ec ==== *)
+require import AllCore List Int IntDiv CoreMap Real Number.
+
+from Jasmin require import JModel.
+from JazzEC require import Array400 Array384 Array256 Array128 Array64 Array32 Array16 Array4 Array8.
+from JazzEC require import WArray512 WArray32 WArray16.
+
+require import W16extra.
+require import AVX2_Ops NTT_avx2 NTT_avx2_poly Fq_avx2 MLKEM_avx2_auxlemmas.
+require import Fq NTT_Fq MLKEMFCLib.
+
+
+from JazzEC require import Jkem_avx2.
+
+from Spec require import GFq Rq Serialization VecMat Correctness.
+
+theory MLKEM_PolyAVX.
+
+import GFq.
+import Fq.
+import SignedReductions_W16.
+import Zq.
+import ZModP.
+import Fq_avx2.
+import NTT_Avx2.
+import Serialization VecMat.
+
+lemma poly_add_corr_h _a _b ab bb :
+      0 <= ab <= 6 => 0 <= bb <= 3 =>
+      hoare[ Mprevec.poly_add2 :
+           _a = lift_array256 rp /\
+           _b = lift_array256 bp /\
+           signed_bound_cxq rp 0 256 ab /\
+           signed_bound_cxq bp 0 256 bb
+           ==>
+           signed_bound_cxq res 0 256 (ab + bb) /\
+           forall k, 0 <= k < 256 =>
+             incoeff (to_sint res.[k]) = _a.[k] + _b.[k]].
+proof. 
+  move => [ab_lb ab_ub] [bb_lb bb_ub].
+  proc.
+  sp.
+  while (0 <= i <= 16 /\
+           (forall k, 16*i <= k < 256 => incoeff (to_sint rp.[k]) = _a.[k]) /\
+           _b = lift_array256 bp /\
+           signed_bound_cxq rp (16*i) 256 ab /\
+           signed_bound_cxq bp 0 256 bb /\
+           signed_bound_cxq rp 0 (16*i) (ab + bb) /\
+           (forall k, 0 <= k < (16*i) =>
+             incoeff (to_sint rp.[k]) = _a.[k] + _b.[k])); last first.
+  auto => />.
+  move => &hr signed_bound_a signed_bound_b.
+  do split; 1..3:by smt(Array256.initiE Array256.mapiE).
+  move => i rp i_tlb i_lb i_ub _ _.
+  have ->: i = 16. by move : i_tlb i_ub => /#.
+  move => -> /=.
+  smt().
+
+  inline Ops.iVPADD_16u16.
+  wp; skip.
+  move => &hr [#] i_lb i_ub _a_def _b_def sgnd_bnd_hrp_a sgnd_bnd_bp sgnd_bnd_lrp_ab lrp_def i_tub />.
+  rewrite mulzDr /=.
+  do split; first 2 by move : i_lb i_tub => /#.
+  move => k k_lb k_ub.
+  rewrite lezNgt in k_lb.
+  rewrite filliE 1:/# k_lb /=.
+  rewrite -lezNgt in k_lb.
+  rewrite -_a_def 1:/# 1:// /=.
+
+  rewrite /signed_bound_cxq => k [k_lb k_ub].
+  rewrite lezNgt in k_lb.
+  rewrite filliE 1:/# k_lb /=.
+  rewrite -lezNgt in k_lb.
+  move : sgnd_bnd_hrp_a => /#.
+
+  rewrite /signed_bound_cxq => k [k_lb k_ub].
+  rewrite filliE 1:/# /= initiE 1:/# /=.
+  case (16 * i{hr} <= k) => k_tlb.
+    + rewrite k_ub /=.
+      do rewrite lift2poly_iso 1..2://.
+      move : (add_corr_qv rp{hr}.[k] bp{hr}.[k] _a.[k] _b.[k] 6 3 _ _ _ _ _ _) => />;
+        1,2:by smt(Array256.initiE Array256.mapiE Array256.tP).
+      rewrite /signed_bound_cxq in sgnd_bnd_hrp_a.
+      move : (sgnd_bnd_hrp_a k) ab_lb ab_ub.
+      rewrite k_tlb /=. by smt().
+
+      rewrite /signed_bound_cxq in sgnd_bnd_bp.
+      move : (sgnd_bnd_bp k) bb_lb bb_ub.
+      rewrite k_lb /=. by smt().
+
+
+      move => rp_bp_def bp_lb bp_ub.
+
+      rewrite to_sintD_small => />.
+        move : (sgnd_bnd_hrp_a k _); first by smt().
+        move : (sgnd_bnd_bp k _); first by smt().
+        smt().
+      move : (sgnd_bnd_hrp_a k _) (sgnd_bnd_bp k _) => /#.
+  + simplify.
+    rewrite /signed_bound_cxq /b16 in sgnd_bnd_lrp_ab.
+    rewrite (sgnd_bnd_lrp_ab k) 1:/#.
+
+  move => k k_lb k_ub.
+  rewrite filliE 1:/# /= initiE 1:/# /=.
+  case (16 * i{hr} <= k) => k_tlb.
+    + rewrite k_ub /=.
+      do (rewrite lift2poly_iso 1..2:// /=).
+      rewrite to_sintD_small => />.
+        move : (sgnd_bnd_hrp_a k _); first by smt().
+        move : (sgnd_bnd_bp k _); first by smt().
+        smt().
+      rewrite incoeffD.
+      rewrite _a_def 1:/#; congr.
+      rewrite /lift_array256 in _b_def.
+      rewrite _b_def mapiE 1:/# //=.
+    + simplify.
+      rewrite -ltzNge in k_tlb.
+      rewrite lrp_def 1..2://.
+qed.
+
+lemma poly_add_ll : islossless Mprevec.poly_add2.
+proof. 
+  proc; while (0<= i <= 16) (16 - i).
+  auto => />.
+  inline Ops.iVPADD_16u16.
+  auto => />.
+  smt().
+  auto => />.
+  smt().
+qed.
+
+lemma poly_add_corr _a _b ab bb :
+    0 <= ab <= 6 => 0 <= bb <= 3 =>  
+      phoare[ Mprevec.poly_add2 :
+           _a = lift_array256 rp /\
+           _b = lift_array256 bp /\
+           signed_bound_cxq rp 0 256 ab /\
+           signed_bound_cxq bp 0 256 bb 
+           ==>
+           signed_bound_cxq res 0 256 (ab + bb) /\ 
+           forall k, 0 <= k < 256 =>
+              incoeff (to_sint res.[k]) = _a.[k] + _b.[k]] = 1%r
+   by move => abb bbb; conseq poly_add_ll (poly_add_corr_h _a _b ab bb abb bbb).
+
+lemma poly_sub_corr_h _a _b ab bb :
+    0 <= ab <= 4 => 0 <= bb <= 4 =>
+      hoare[ Mprevec.poly_sub :
+           _a = lift_array256 ap /\
+           _b = lift_array256 bp /\
+           signed_bound_cxq ap 0 256 ab /\
+           signed_bound_cxq bp 0 256 bb
+           ==>
+           signed_bound_cxq res 0 256 (ab + bb) /\
+           forall k, 0 <= k < 256 =>
+              incoeff (to_sint res.[k]) = _a.[k] - _b.[k]].
+proof. 
+  move => [ab_lb ab_ub] [bb_lb bb_ub].
+  proc.
+  while (0 <= i <= 16 /\
+           _a = lift_array256 ap /\
+           _b = lift_array256 bp /\
+           signed_bound_cxq ap 0 256 ab /\
+           signed_bound_cxq bp 0 256 bb /\
+           signed_bound_cxq rp 0 (16*i) (ab + bb) /\
+           forall k, 0 <= k < (16*i) =>
+              incoeff (to_sint rp.[k]) = _a.[k] - _b.[k]
+  ); first last.
+  auto => />.
+  move => &hr signed_bound_a signed_bound_b.
+  do split; first 3 by smt().
+
+  inline Ops.iVPSUB_16u16.
+  wp; skip.
+  move => &hr [#] i_lb i_ub _a_def _b_def sgnd_bnd_hap_a sgnd_bnd_bp sgnd_bnd_lrp_ab lrp_def i_tub />.
+
+  rewrite mulzDr /=.
+  do split; first 2 by move : i_lb i_tub => /#.
+  
+  rewrite /signed_bound_cxq => k [k_lb k_ub].
+  rewrite filliE 1:/# /=.
+  case (16 * i{hr} <= k) => k_tlb.
+    + rewrite k_ub /= initiE 1:/# /=.
+      do (rewrite lift2poly_iso 1:/# 1:/#).
+      rewrite to_sintB_small => />.
+        move : (sgnd_bnd_hap_a k _) (sgnd_bnd_bp k _) => /#.
+        move : (sgnd_bnd_hap_a k _) (sgnd_bnd_bp k _) => /#.
+    + simplify. rewrite -ltzNge in k_tlb.
+      rewrite /signed_bound_cxq /b16 in sgnd_bnd_lrp_ab.
+      rewrite (sgnd_bnd_lrp_ab k _); first by rewrite k_lb k_tlb.
+
+  move => k k_lb k_ub.
+  rewrite filliE 1:/# /= initiE 1:/# /=.
+  case (16 * i{hr} <= k) => k_tlb.
+    + rewrite k_ub /=.
+      do (rewrite lift2poly_iso //=).
+      rewrite to_sintB_small => />.
+        move : (sgnd_bnd_hap_a k _) (sgnd_bnd_bp k _) => /#.
+      rewrite incoeffB.
+      rewrite _b_def _a_def /lift_array256.
+      rewrite mapiE 1:/# mapiE 1:/# //=.
+    + simplify.
+      rewrite -ltzNge in k_tlb.
+      rewrite lrp_def //=.
+qed.
+
+lemma poly_sub_ll : islossless Mprevec.poly_sub.
+proof. 
+  proc; while (0<= i <= 16) (16 - i); auto => />.
+  inline Ops.iVPSUB_16u16.
+  auto => />; smt().
+  auto => />; smt().
+qed.
+
+lemma poly_sub_corr _a _b ab bb :
+    0 <= ab <= 4 => 0 <= bb <= 4 =>  
+      phoare[ Mprevec.poly_sub :
+           _a = lift_array256 ap /\
+           _b = lift_array256 bp /\
+           signed_bound_cxq ap 0 256 ab /\
+           signed_bound_cxq bp 0 256 bb 
+           ==>
+           signed_bound_cxq res 0 256 (ab + bb) /\ 
+           forall k, 0 <= k < 256 =>
+              incoeff (to_sint res.[k]) = _a.[k] - _b.[k]] = 1%r
+  by move => *; conseq poly_sub_ll (poly_sub_corr_h _a _b ab bb _ _).
+
+require import NTTAlgebra.
+lemma poly_reduce_corr_h (ap: coeff Array256.t):
+     hoare[ Mprevec.poly_reduce :
+          ap = lift_array256 rp ==>
+          ap = lift_array256 res /\
+          forall k, 0 <= k < 256 => bpos16 res.[k] (2*q)].
+proof. 
+  proc.
+  while (0 <= i <= 16 /\
+         (forall k, 0 <= k < 256 => ap.[k] = incoeff (to_sint rp.[k])) /\
+         (forall k, 0 <= k < 16 * i => bpos16 rp.[k] (2*q)) /\
+         (forall k, 0 <= k < 16 => qx16.[k] = Jkem_avx2.jqx16.[k]) /\
+         (forall k, 0 <= k < 16 => vx16.[k] = Jkem_avx2.jvx16.[k])); last first.
+  wp. skip.
+  move => &hr ap_def />.
+  do split.
+  rewrite ap_def /lift_array256 => k k_lb k_ub.
+  rewrite mapiE 1:/# //=.
+  
+  smt().
+  
+  move => k k_lb k_ub.
+  rewrite /lift2poly initiE => />.
+  rewrite /get256_direct => />.
+  rewrite k_lb k_ub => /=.
+  rewrite W32u8.Pack.initiE. move : k_lb k_ub => /#.
+  rewrite W32u8.Pack.initiE. move : k_lb k_ub => /#.
+  rewrite initiE. move : k_lb k_ub => /#. simplify.
+  rewrite initiE. move : k_lb k_ub => /#. simplify.
+  rewrite (_:(2*k + 1) %/2 = 2*k %/ 2).
+    smt().
+  rewrite (_: 2*k %% 2 = 0).
+    smt().
+  rewrite (_: (2*k + 1) %% 2 = 1).
+    smt().
+  rewrite pack2_bits8.
+  smt().
+  
+  move => k k_lb k_ub.
+  rewrite /lift2poly initiE => />.
+  rewrite /get256_direct => />.
+  rewrite k_lb k_ub => /=.
+  rewrite W32u8.Pack.initiE. move : k_lb k_ub => /#.
+  rewrite W32u8.Pack.initiE. move : k_lb k_ub => /#.
+  rewrite initiE. move : k_lb k_ub => /#. simplify.
+  rewrite initiE. move : k_lb k_ub => /#. simplify.
+  rewrite (_:(2*k + 1) %/2 = 2*k %/ 2).
+    smt().
+  rewrite (_: 2*k %% 2 = 0).
+    smt().
+  rewrite (_: (2*k + 1) %% 2 = 1).
+    smt().
+  rewrite pack2_bits8.
+  smt().
+  
+  move => i rpu i_tlb i_lb i_ub.
+  have ->: i=16. by move : i_tlb i_ub => /#.
+  simplify.
+  move => ap_eq_rpu rpu_bnds jqx16_def vx16_def.
+  split.
+    + apply Array256.ext_eq => x x_i.
+      rewrite /lift_array256 mapiE 1:x_i /= ap_eq_rpu 1:x_i //=.
+    + move : rpu_bnds => /#.
+  
+  wp; sp; ecall (Fq_avx2.barret_red16x_corr_hh (Fq_avx2.lift_array16 r)). auto => />.
+  move => &hr i_lb i_rub rp_sbred rp_eq__rp qx16_def vx16_def i_ub result red16x_bred.
+  split; first by move : i_lb i_ub => /#.
+  pose rp_sub := ((Fq_avx2.lift_array16
+                       (lift2poly
+                          (get256 ((init16 ("_.[_]" rp{hr})))%WArray512 i{hr})))).
+  split.
+  move => k k_lb k_ub.
+  rewrite filliE 1:/# /=.
+  case (16 * i{hr} <= k && k < 16 * i{hr} + 16) => k_si.
+    + have bred := (BREDCp_corr rp_sub.[k %% 16] 26 _ _ _ _ _ _);
+        1..4,6: smt(qE pow2_16).
+        rewrite /rp_sub /lift_array16 mapiE 1:/# /= /R.
+        move : W16.to_sint_cmp => /#.
+      move : bred => [bred_i bred_cgr].
+      rewrite red16x_bred 1:/#.
+      rewrite eq_incoeff in bred_cgr.
+      rewrite bred_cgr.
+      rewrite /lift_array16 /= mapiE 1:/# /= lift2poly_iso //.
+      rewrite (rp_sbred k _) //.
+    + rewrite (rp_sbred k _) //.
+  rewrite mulzDr mulz1 => k k_lb k_ub.
+  rewrite filliE // 1:/# k_ub /=.
+  case (16 * i{hr} <= k) => k_tlb.
+    + have bred := (BREDCp_corr rp_sub.[k %% 16] 26 _ _ _ _ _ _);
+        1..4,6: smt(qE pow2_16).
+        rewrite /rp_sub /lift_array16 mapiE 1:/# /= /R.
+        move : W16.to_sint_cmp => /#.
+        move : bred; rewrite andabP; move => [[bred_lb bred_ub] bred_cgr].
+        (* move : bred => /andabP [[bred_lb bred_ub] bred_cgr]. *)
+        rewrite red16x_bred 1:/# -/rp_sub bred_lb bred_ub //=.
+    + rewrite -ltzNge in k_tlb.
+      move : (rp_eq__rp k); rewrite k_lb k_tlb /= => /#.
+qed.
+
+lemma poly_reduce_ll:
+  islossless Mprevec.poly_reduce.
+proof. 
+  proc; while(0 <= i <= 16) (16 - i);
+    move => *; inline *; auto => />.
+  move => &hr i_lb i_ub i_tub.
+  split.
+  move : i_lb i_tub => /#.
+  smt().
+  smt().
+qed.
+
+lemma poly_reduce_corr ap:
+  phoare[ Mprevec.poly_reduce :
+        ap = lift_array256 rp ==>
+        ap = lift_array256 res /\
+        forall k, 0 <= k < 256 => bpos16 res.[k] (2*q)] = 1%r.
+proof.  by conseq poly_reduce_ll (poly_reduce_corr_h ap). qed.
+
+lemma poly_frommont_corr_h ap:
+  hoare[ Mprevec.poly_frommont :
+       ap = map W16.to_sint rp ==>
+       map W16.to_sint res = map (fun x => SREDC (x * ((Ring.IntID.(^) SignedReductions.R 2) %% q))) ap].
+proof. 
+  proc.
+  while(0 <= i <= 16 /\ aux = 16 /\
+        (forall k, 0 <= k < 16 => dmontx16.[k] = W16.of_int 1353) /\
+        (forall k, 0 <= k < 16 => qx16.[k] = W16.of_int 3329) /\
+        (forall k, 0 <= k < 16 => qinvx16.[k] = W16.of_int (-3327)) /\
+        (forall k, 0 <= k < 16 * i => W16.to_sint rp.[k] = SREDC (ap.[k] * ((Ring.IntID.(^) SignedReductions.R 2) %% q))) /\
+        (forall k, 16 * i <= k < 256 => W16.to_sint rp.[k] = ap.[k])); last first.
+  auto => />.
+  move => &hr.
+  do split.
+  
+  move => k k_lb k_ub.
+  rewrite /lift2poly //=.
+  rewrite initiE //.
+  rewrite /get256_direct //=.
+  rewrite k_lb k_ub /=.
+  rewrite W32u8.Pack.initiE //=. move : k_lb k_ub => /#.
+  rewrite W32u8.Pack.initiE //=. move : k_lb k_ub => /#.
+  rewrite WArray32.initiE //=. move : k_lb k_ub => /#.
+  rewrite WArray32.initiE //=. move : k_lb k_ub => /#.
+  rewrite (_: (2 * k + 1) %/ 2 = (2 * k) %/ 2).
+    by smt().
+  rewrite (_: 2 * k %% 2 = 0).
+    by smt().
+  rewrite (_: (2 * k + 1) %% 2 = 1).
+    by smt().
+  rewrite pack2_bits8.
+  rewrite /(Jkem_avx2.jdmontx16) => />.
+  rewrite initiE => />. move : k_lb k_ub => /#.
+  smt().
+  
+  move => k k_lb k_ub.
+  rewrite /lift2poly //=.
+  rewrite initiE //.
+  rewrite /get256_direct //=.
+  rewrite k_lb k_ub /=.
+  rewrite W32u8.Pack.initiE //=. move : k_lb k_ub => /#.
+  rewrite W32u8.Pack.initiE //=. move : k_lb k_ub => /#.
+  rewrite WArray32.initiE //=. move : k_lb k_ub => /#.
+  rewrite WArray32.initiE //=. move : k_lb k_ub => /#.
+  rewrite (_: (2 * k + 1) %/ 2 = (2 * k) %/ 2).
+    by smt().
+  rewrite (_: 2 * k %% 2 = 0).
+    by smt().
+  rewrite (_: (2 * k + 1) %% 2 = 1).
+    by smt().
+  rewrite pack2_bits8.
+  rewrite /(Jkem_avx2.jqx16) => />.
+  rewrite initiE => />. move : k_lb k_ub => /#.
+  smt().
+  
+  move => k k_lb k_ub.
+  rewrite /lift2poly //=.
+  rewrite initiE //.
+  rewrite /get256_direct //=.
+  rewrite k_lb k_ub /=.
+  rewrite W32u8.Pack.initiE //=. move : k_lb k_ub => /#.
+  rewrite W32u8.Pack.initiE //=. move : k_lb k_ub => /#.
+  rewrite WArray32.initiE //=. move : k_lb k_ub => /#.
+  rewrite WArray32.initiE //=. move : k_lb k_ub => /#.
+  rewrite (_: (2 * k + 1) %/ 2 = (2 * k) %/ 2).
+    by smt().
+  rewrite (_: 2 * k %% 2 = 0).
+    by smt().
+  rewrite (_: (2 * k + 1) %% 2 = 1).
+    by smt().
+  rewrite pack2_bits8.
+  rewrite initiE => />. move : k_lb k_ub => /#.
+  smt().
+  
+  smt().
+  smt(Array256.mapiE).
+  move => i rp i_tlb i_lb i_ub jdmontx16_def jqinvx16_def jqx16_def rp_sredc rp_sint_rp0.
+  apply Array256.ext_eq.
+  move => x x_bnds.
+  do rewrite mapiE //=.
+  rewrite -lezNgt in i_tlb.
+  rewrite (rp_sredc x).
+  move : i_tlb i_ub x_bnds => /#.
+  rewrite mapiE //.
+  sp. wp.
+  ecall (Fq_avx2.fqmulx16_corr_hh (Fq_avx2.lift_array16 t) (Fq_avx2.lift_array16 dmontx16)).
+  auto => />.
+  move => &hr i_lb i_ub dmontx16_def qx16_def qinvx16_def rp_sredc rp_eq_ap i_tub result result_def.
+  split.
+  move : i_lb i_tub => /#.
+  
+  rewrite fillE.
+  split.
+  
+  move => k k_lb k_ub.
+  have k_mb: 0 <= k %% 16 < 16.
+    by smt().
+  rewrite initiE //=; first by move : k_lb k_ub i_tub => /#.
+  
+  case (k < 16 * i{hr}).
+    + move => /ltzNge k_tub.
+      rewrite k_tub /=.
+      apply (rp_sredc k); by move : k_lb k_tub => /#.
+    + move => /lezNgt k_tlb.
+      rewrite mulzDr mulz1 in k_ub.
+      rewrite k_tlb k_ub => /=.
+      rewrite result_def //.
+      rewrite /lift_array16 mapiE //= lift2poly_iso // mapiE //=.
+      rewrite dmontx16_def // of_sintK => />.
+      rewrite rp_eq_ap //. rewrite k_tlb; move : k_ub i_tub => /#.
+      rewrite /R qE /=.
+      congr.
+      rewrite /smod //=.
+  
+  move => k k_lb k_ub.
+  rewrite initiE //=; first by move : k_lb i_lb k_ub => /#.
+  rewrite mulzDr mulz1 lezNgt in k_lb.
+  rewrite k_lb /=.
+  apply rp_eq_ap; by move : k_lb k_ub => /#.
+qed.
+
+lemma poly_frommont_ll : islossless  Mprevec.poly_frommont.
+proof. 
+  proc.
+  auto => />.
+  cfold 4. wp; while (0 <= i <= 16) (16 - i).
+  + move => *; inline*; auto => />. smt().
+  + inline *; wp; auto => /> /#.
+qed.
+
+lemma poly_frommont_corr ap:
+  phoare[ Mprevec.poly_frommont :
+       ap = map W16.to_sint rp ==>
+       map W16.to_sint res = map (fun x => SREDC (x * ((Ring.IntID.(^) SignedReductions.R 2) %% q))) ap] = 1%r
+ by conseq poly_frommont_ll (poly_frommont_corr_h ap) => />.
+
+op lift_array16 (p: W16.t Array16.t) =
+  Array16.map (fun x => incoeff (W16.to_sint x)) p.
+
+lemma shuffle8_corr_h _a _b:
+      hoare[ Mprevec.shuffle8 :
+           _a = a /\ _b = b
+           ==>
+           res.`1 = (shuf8 _a _b).`1 /\
+           res.`2 = (shuf8 _a _b).`2].
+proof.
+  proc.
+  wp; inline *; auto => />.
+  split.
+    + rewrite /shuf8 => />.
+      rewrite -ext_eq_all /all_eq //=.
+    + rewrite /shuf8 => />.
+      rewrite -ext_eq_all /all_eq //=.
+qed.
+
+lemma shuffle4_corr_h _a _b:
+      hoare[ Mprevec.shuffle4 :
+           _a = a /\ _b = b
+           ==>
+           res.`1 = (shuf4 _a _b).`1 /\
+           res.`2 = (shuf4 _a _b).`2].
+proof.
+  proc.
+  wp; inline *; auto => />.
+  split.
+    + rewrite /shuf4 => />.
+      rewrite -ext_eq_all /all_eq //=.
+    + rewrite /shuf4 => />.
+      rewrite -ext_eq_all /all_eq //=.
+qed.
+
+lemma shuffle2_corr_h _a _b:
+      hoare[ Mprevec.shuffle2 :
+           _a = a /\ _b = b
+           ==>
+           res.`1 = (shuf2 _a _b).`1 /\
+           res.`2 = (shuf2 _a _b).`2].
+proof.
+  proc.
+  wp; inline *; auto => />.
+  split.
+    + rewrite /shuf2 => />.
+      rewrite -ext_eq_all /all_eq //=.
+    + rewrite /shuf2 /f16u16_t4u64 /f4u64_t16u16 /lift_array16 => />.
+      rewrite -ext_eq_all /all_eq => />.
+      rewrite /W8.int_bit => />.
+      rewrite shr_shrw 1:/#.
+      rewrite wlsrE => />.
+      do split; first 8 by apply W16.all_eq_eq.
+qed.
+
+lemma shuffle1_corr_h _a _b:
+      hoare[ Mprevec.shuffle1 :
+           _a = a /\ _b = b
+           ==>
+           res.`1 = (shuf1 _a _b).`1 /\
+           res.`2 = (shuf1 _a _b).`2].
+proof.
+  proc.
+  wp; inline *; auto => />.
+  rewrite /shuf1 /f8u32_t16u16 /f16u16_t8u32 /lift_array16 => />.
+  do (rewrite -ext_eq_all /all_eq /=).
+  rewrite /W8.int_bit => />.
+  do (rewrite shl_shlw 1:/#; rewrite wlslE => />).
+  do (rewrite shr_shrw 1:/#; rewrite wlsrE => />).
+  do split; first 16 by apply W16.all_eq_eq.
+qed.
+
+end MLKEM_PolyAVX.
+
+(* ==== from MLKEM_Poly_avx2_vec.ec ==== *)
+require import AllCore List Int IntDiv CoreMap.
+
+from Jasmin require import JModel.
+from JazzEC require import Array400 Array256 Array128 Array64 Array32 Array16 Array8 Array4.
+from JazzEC require import WArray800 WArray512 WArray128 WArray64 WArray32 WArray16.
+require import AVX2_Ops.
+from JazzEC require import Jkem_avx2.
+require import MLKEM_avx2_auxlemmas MLKEMFCLib.
+
+
+module Mvec = {
+  proc shuffle8 (a:W256.t, b:W256.t) : W256.t * W256.t = {
+    
+    var r0:W256.t;
+    var r1:W256.t;
+    
+    r0 <@ OpsV.iVPERM2I128_16u16(a, b, (W8.of_int 32));
+    r1 <@ OpsV.iVPERM2I128_16u16(a, b, (W8.of_int 49));
+    return (r0, r1);
+  }
+  
+  proc shuffle4 (a:W256.t, b:W256.t) : W256.t * W256.t = {
+    
+    var r0:W256.t;
+    var r1:W256.t;
+    
+    r0 <@ OpsV.iVPUNPCKL_4u64_16u16(a, b);
+    r1 <@ OpsV.iVPUNPCKH_4u64_16u16(a, b);
+    return (r0, r1);
+  }
+  
+  proc shuffle2 (a:W256.t, b:W256.t) : W256.t * W256.t = {
+    
+    var t0:W256.t;
+    var t1:W256.t;
+    
+    t0 <@ OpsV.iVMOVSLDUP_256_16u16(b);
+    t0 <@ OpsV.iVPBLEND_8u32_16u16(a, t0, (W8.of_int 170));
+    a  <@ OpsV.iVPSRL_4u64(a, (W128.of_int 32));
+    t1 <@ OpsV.iVPBLEND_8u32_16u16(a, b, (W8.of_int 170));
+    return (t0, t1);
+  }
+  
+  proc shuffle1 (a:W256.t, b:W256.t) : W256.t * W256.t = {
+    
+    var r0:W256.t;
+    var r1:W256.t;
+    var t0:W256.t;
+    var t1:W256.t;
+    
+    t0 <@ OpsV.iVPSLL_8u32(b, (W128.of_int 16));
+    r0 <@ OpsV.iVPBLEND_16u16(a, t0, (W8.of_int 170));
+    t1 <@ OpsV.iVPSRL_8u32(a, (W128.of_int 16));
+    r1 <@ OpsV.iVPBLEND_16u16(t1, b, (W8.of_int 170));
+
+    return (r0, r1);
+  }
+
+  proc poly_add2(rp:W16.t Array256.t, bp:W16.t Array256.t) : W16.t Array256.t = {
+    var i:int;
+    var a:W256.t;
+    var b:W256.t;
+    var r:W256.t;
+
+    i <- 0;
+
+    while (i < 16) {
+      a <- (get256_direct (WArray512.init16 (fun i => rp.[i])) (32 * i));
+      b <- (get256_direct (WArray512.init16 (fun i => bp.[i])) (32 * i));
+      r <@ OpsV.iVPADD_16u16(a, b);
+      rp <-
+      Array256.init
+      (WArray512.get16 (WArray512.set256_direct (WArray512.init16 (fun i => rp.[i])) (32 * i) r));
+      i <- i + 1;
+    }
+
+    return (rp);
+  }
+
+  proc poly_sub (rp:W16.t Array256.t, ap:W16.t Array256.t,
+                 bp:W16.t Array256.t) : W16.t Array256.t = {
+    var aux: int;
+
+    var i:int;
+    var a:W256.t;
+    var b:W256.t;
+    var r:W256.t;
+
+    i <- 0;
+    while (i < 16) {
+      a <- (get256_direct (WArray512.init16 (fun i => ap.[i])) (32 * i));
+      b <- (get256_direct (WArray512.init16 (fun i => bp.[i])) (32 * i));
+      r <@ OpsV.iVPSUB_16u16(a, b);
+      rp <-
+      Array256.init
+      (WArray512.get16 (WArray512.set256_direct (WArray512.init16 (fun i => rp.[i])) (32 * i) r));
+      i <- i + 1;
+    }
+    return (rp);
+  }
+
+  proc csubq (r:W256.t, qx16:W256.t) : W256.t = {
+    var t:W256.t;
+
+    r <@ OpsV.iVPSUB_16u16(r, qx16);
+    t <@ OpsV.iVPSRA_16u16(r, (W128.of_int 15));
+    t <@ OpsV.iVPAND_16u16(t,qx16);
+    r <@ OpsV.iVPADD_16u16(t, r);
+
+    return (r);
+  }
+
+  proc poly_csubq (rp:W16.t Array256.t) : W16.t Array256.t = {
+    var aux: int;
+
+    var qx16:W256.t;
+    var i:int;
+    var r:W256.t;
+
+    qx16 <- (get256 (WArray32.init16 (fun i => jqx16.[i])) 0);
+    i <- 0;
+    while (i < 16) {
+      r <- (get256_direct (WArray512.init16 (fun i => rp.[i])) (32 * i));
+      r <@ csubq (r, qx16);
+      rp <-
+      Array256.init
+      (WArray512.get16 (WArray512.set256_direct (WArray512.init16 (fun i => rp.[i])) (32 * i) r));
+      i <- i + 1;
+    }
+    return (rp);
+  }
+
+
+  proc  red16x (r:W256.t, qx16:W256.t, vx16:W256.t) : W256.t = {
+    var x:W256.t;
+
+    x <@ OpsV.iVPMULH_256(r, vx16);
+    x <@ OpsV.iVPSRA_16u16(x, (W128.of_int 10));
+    x <@ OpsV.iVPMULL_16u16(x, qx16);
+    r <@ OpsV.iVPSUB_16u16(r, x);
+    return (r);
+  }
+
+  proc fqmulx16 (a:W256.t, b:W256.t, qx16:W256.t, qinvx16:W256.t) : W256.t = {
+
+    var rd:W256.t;
+    var rhi:W256.t;
+    var rlo:W256.t;
+
+    rhi <@ OpsV.iVPMULH_256(a, b);
+    rlo <@ OpsV.iVPMULL_16u16(a, b);
+    rlo <@ OpsV.iVPMULL_16u16(rlo, qinvx16);
+    rlo <@ OpsV.iVPMULH_256(rlo, qx16);
+    rd <@ OpsV.iVPSUB_16u16(rhi, rlo);
+    return (rd);
+  }
+
+  proc poly_reduce (rp:W16.t Array256.t) : W16.t Array256.t = {
+    var aux: int;
+
+    var qx16:W256.t;
+    var vx16:W256.t;
+    var i:int;
+    var r:W256.t;
+
+    qx16 <- (get256 (WArray32.init16 (fun i => jqx16.[i])) 0);
+    vx16 <- (get256 (WArray32.init16 (fun i => jvx16.[i])) 0);
+    i <- 0;
+    while (i < 16) {
+      r <- (get256_direct (WArray512.init16 (fun i => rp.[i])) (32 * i));
+      r <@ red16x (r, qx16, vx16);
+      rp <-
+      Array256.init
+      (WArray512.get16 (WArray512.set256_direct (WArray512.init16 (fun i => rp.[i])) (32 * i) r));
+      i <- i + 1;
+    }
+    return (rp);
+  }
+
+  proc poly_frommont (rp:W16.t Array256.t) : W16.t Array256.t = {
+    var aux: int;
+
+    var x16p:W16.t Array16.t;
+    var qx16:W256.t;
+    var qinvx16:W256.t;
+    var dmontx16:W256.t;
+    var i:int;
+    var t:W256.t;
+    x16p <- witness;
+    x16p <- jqx16;
+    qx16 <- (get256 (WArray32.init16 (fun i => jqx16.[i])) 0);
+    x16p <- jqinvx16;
+    qinvx16 <- (get256 (WArray32.init16 (fun i => jqinvx16.[i])) 0);
+    x16p <- jdmontx16;
+    dmontx16 <- (get256 (WArray32.init16 (fun i => jdmontx16.[i])) 0);
+    aux <- (256 %/ 16);
+    i <- 0;
+    while (i < aux) {
+      t <- (get256 (WArray512.init16 (fun i => rp.[i])) i);
+      t <@ fqmulx16 (t, dmontx16, qx16, qinvx16);
+      rp <-
+      Array256.init
+      (WArray512.get16 (WArray512.set256 (WArray512.init16 (fun i => rp.[i])) i t));
+      i <- i + 1;
+    }
+    return (rp);
+  }
+
+  proc schoolbook (ap:W16.t Array32.t, bp:W16.t Array32.t, zeta_0:W256.t,
+                   qx16:W256.t, qinvx16:W256.t, sign:int) : W256.t * W256.t *
+                                                            W256.t * W256.t = {
+
+    var x0:W256.t;
+    var x1:W256.t;
+    var y0:W256.t;
+    var y1:W256.t;
+    var b:W256.t;
+    var d:W256.t;
+    var a:W256.t;
+    var c:W256.t;
+    var bdlo:W256.t;
+    var bdhi:W256.t;
+    var bclo:W256.t;
+    var bchi:W256.t;
+    var adlo:W256.t;
+    var adhi:W256.t;
+    var aclo:W256.t;
+    var achi:W256.t;
+    var bd:W256.t;
+    var rbdlo:W256.t;
+    var rbdhi:W256.t;
+    var bc0:W256.t;
+    var bc1:W256.t;
+    var ad0:W256.t;
+    var ad1:W256.t;
+    var ac0:W256.t;
+    var ac1:W256.t;
+    var rbd0:W256.t;
+    var rbd1:W256.t;
+
+    b <- (get256_direct (WArray64.init16 (fun i => ap.[i])) (32 * 1));
+    d <- (get256_direct (WArray64.init16 (fun i => bp.[i])) (32 * 1));
+    a <- (get256_direct (WArray64.init16 (fun i => ap.[i])) (32 * 0));
+    c <- (get256_direct (WArray64.init16 (fun i => bp.[i])) (32 * 0));
+    bdlo <@ OpsV.iVPMULL_16u16(b, d);
+    bdhi <@ OpsV.iVPMULH_256(b, d);
+    bclo <@ OpsV.iVPMULL_16u16(b, c);
+    bchi <@ OpsV.iVPMULH_256(b, c);
+    adlo <@ OpsV.iVPMULL_16u16(a, d);
+    adhi <@ OpsV.iVPMULH_256(a, d);
+    aclo <@ OpsV.iVPMULL_16u16(a, c);
+    achi <@ OpsV.iVPMULH_256(a, c);
+    bdlo <@ OpsV.iVPMULL_16u16(bdlo, qinvx16);
+    bdlo <@ OpsV.iVPMULH_256(bdlo, qx16);
+    bd <@ OpsV.iVPSUB_16u16(bdhi, bdlo);
+    rbdlo <@ OpsV.iVPMULL_16u16(zeta_0, bd);
+    rbdhi <@ OpsV.iVPMULH_256(zeta_0, bd);
+    bc0 <@ OpsV.iVPUNPCKL_16u16(bclo, bchi);
+    bc1 <@ OpsV.iVPUNPCKH_16u16(bclo, bchi);
+    ad0 <@ OpsV.iVPUNPCKL_16u16(adlo, adhi);
+    ad1 <@ OpsV.iVPUNPCKH_16u16(adlo, adhi);
+    ac0 <@ OpsV.iVPUNPCKL_16u16(aclo, achi);
+    ac1 <@ OpsV.iVPUNPCKH_16u16(aclo, achi);
+    rbd0 <@ OpsV.iVPUNPCKL_16u16(rbdlo, rbdhi);
+    rbd1 <@ OpsV.iVPUNPCKH_16u16(rbdlo, rbdhi);
+    if ((sign = 0)) {
+      x0 <@ OpsV.iVPADD_8u32(ac0, rbd0);
+      x1 <@ OpsV.iVPADD_8u32(ac1, rbd1);
+    } else {
+      x0 <@ OpsV.iVPSUB_8u32(ac0, rbd0);
+      x1 <@ OpsV.iVPSUB_8u32(ac1, rbd1);
+    }
+    y0 <@ OpsV.iVPADD_8u32(bc0, ad0);
+    y1 <@ OpsV.iVPADD_8u32(bc1, ad1);
+    return (x0, x1, y0, y1);
+  }
+
+  proc basemul_red (a0:W256.t, a1:W256.t, b0:W256.t, b1:W256.t, qx16:W256.t,
+                    qinvx16:W256.t) : W256.t * W256.t = {
+
+    var zero:W256.t;
+    var y:W256.t;
+    var z:W256.t;
+    var x:W256.t;
+
+    zero <- W256.zero ;
+    y <@ OpsV.iVPBLEND_16u16(a0, zero, (W8.of_int 170));
+    z <@ OpsV.iVPBLEND_16u16(a1, zero, (W8.of_int 170));
+    a0 <@ OpsV.iVPSRL_8u32(a0, (W128.of_int 16));
+    a1 <@ OpsV.iVPSRL_8u32(a1, (W128.of_int 16));
+    z <@ OpsV.iVPACKUS_8u32(y, z);
+    a0 <@ OpsV.iVPACKUS_8u32(a0, a1);
+    y <@ OpsV.iVPBLEND_16u16(b0, zero, (W8.of_int 170));
+    x <@ OpsV.iVPBLEND_16u16(b1, zero, (W8.of_int 170));
+    b0 <@ OpsV.iVPSRL_8u32(b0, (W128.of_int 16));
+    b1 <@ OpsV.iVPSRL_8u32(b1, (W128.of_int 16));
+    y <@ OpsV.iVPACKUS_8u32(y, x);
+    b0 <@ OpsV.iVPACKUS_8u32(b0, b1);
+    z <@ OpsV.iVPMULL_16u16(z, qinvx16);
+    y <@ OpsV.iVPMULL_16u16(y, qinvx16);
+    z <@ OpsV.iVPMULH_256(z, qx16);
+    y <@ OpsV.iVPMULH_256(y, qx16);
+    a0 <@ OpsV.iVPSUB_16u16(a0, z);
+    b0 <@ OpsV.iVPSUB_16u16(b0, y);
+    return (a0, b0);
+  }
+
+  proc basemul32x (rp:W16.t Array64.t, ap:W16.t Array64.t,
+                   bp:W16.t Array64.t, zeta_0:W256.t, qx16:W256.t,
+                   qinvx16:W256.t) : W16.t Array64.t = {
+
+    var x0:W256.t;
+    var x1:W256.t;
+    var y0:W256.t;
+    var y1:W256.t;
+
+    (x0, x1, y0, y1) <@ schoolbook ((Array32.init (fun i => ap.[0 + i])),
+    (Array32.init (fun i => bp.[0 + i])), zeta_0, qx16, qinvx16, 0);
+    (x0, x1) <@ basemul_red (x0, x1, y0, y1, qx16, qinvx16);
+    rp <-
+    Array64.init
+    (WArray128.get16 (WArray128.set256_direct (WArray128.init16 (fun i => rp.[i])) (32 * 0) x0));
+    rp <-
+    Array64.init
+    (WArray128.get16 (WArray128.set256_direct (WArray128.init16 (fun i => rp.[i])) (32 * 1) x1));
+    (x0, x1, y0, y1) <@ schoolbook ((Array32.init (fun i => ap.[32 + i])),
+    (Array32.init (fun i => bp.[32 + i])), zeta_0, qx16, qinvx16, 1);
+    (x0, x1) <@ basemul_red (x0, x1, y0, y1, qx16, qinvx16);
+    rp <-
+    Array64.init
+    (WArray128.get16 (WArray128.set256_direct (WArray128.init16 (fun i => rp.[i])) (32 * 2) x0));
+    rp <-
+    Array64.init
+    (WArray128.get16 (WArray128.set256_direct (WArray128.init16 (fun i => rp.[i])) (32 * 3) x1));
+    return (rp);
+  }
+
+  proc poly_basemul (rp:W16.t Array256.t, ap:W16.t Array256.t,
+                     bp:W16.t Array256.t) : W16.t Array256.t = {
+    var aux: W16.t Array64.t;
+
+    var qx16:W256.t;
+    var qinvx16:W256.t;
+    var zeta_0:W256.t;
+
+    qx16 <- (get256_direct (WArray32.init16 (fun i => jqx16.[i])) 0);
+    qinvx16 <- (get256_direct (WArray32.init16 (fun i => jqinvx16.[i])) 0);
+    zeta_0 <-
+    (get256_direct (WArray800.init16 (fun i => jzetas_exp.[i])) 304);
+    aux <@ basemul32x ((Array64.init (fun i => rp.[0 + i])),
+    (Array64.init (fun i => ap.[0 + i])),
+    (Array64.init (fun i => bp.[0 + i])), zeta_0, qx16, qinvx16);
+    rp <- Array256.init
+          (fun i => if 0 <= i < 0 + 64 then aux.[i-0] else rp.[i]);
+    zeta_0 <-
+    (get256_direct (WArray800.init16 (fun i => jzetas_exp.[i])) 368);
+    aux <@ basemul32x ((Array64.init (fun i => rp.[64 + i])),
+    (Array64.init (fun i => ap.[64 + i])),
+    (Array64.init (fun i => bp.[64 + i])), zeta_0, qx16, qinvx16);
+    rp <- Array256.init
+          (fun i => if 64 <= i < 64 + 64 then aux.[i-64] else rp.[i]);
+    zeta_0 <-
+    (get256_direct (WArray800.init16 (fun i => jzetas_exp.[i])) 696);
+    aux <@ basemul32x ((Array64.init (fun i => rp.[128 + i])),
+    (Array64.init (fun i => ap.[128 + i])),
+    (Array64.init (fun i => bp.[128 + i])), zeta_0, qx16, qinvx16);
+    rp <- Array256.init
+          (fun i => if 128 <= i < 128 + 64 then aux.[i-128] else rp.[i]);
+    zeta_0 <-
+    (get256_direct (WArray800.init16 (fun i => jzetas_exp.[i])) 760);
+    aux <@ basemul32x ((Array64.init (fun i => rp.[192 + i])),
+    (Array64.init (fun i => ap.[192 + i])),
+    (Array64.init (fun i => bp.[192 + i])), zeta_0, qx16, qinvx16);
+    rp <- Array256.init
+          (fun i => if 192 <= i < 192 + 64 then aux.[i-192] else rp.[i]);
+    return (rp);
+  }
+
+}.
+
+theory MLKEM_PolyAVXVec.
+
+equiv eq_poly_add2:
+  Mprevec.poly_add2 ~ Mvec.poly_add2: ={rp, bp} ==> ={res}.
+proof.
+  proc.
+  while(={rp, bp, i} /\ 0 <= i{1}).
+  wp.
+  call eq_iVPADD_16u16.
+  wp. skip. rewrite /is16u16 => />. move => &1 i_lb i_ub.
+  do split.
+  rewrite /lift2poly; simplify; rewrite pack16_bits16; trivial.
+  rewrite /lift2poly; simplify; rewrite pack16_bits16; trivial.
+  move => rp_eq bp_eq result_L.
+  split.
+  rewrite fillE //=.
+  apply Array256.ext_eq.
+  move => x x_i.
+  have x_mb: 0 <= x %% 16 < 16.
+    by smt().
+  do rewrite initiE //=.
+  rewrite set_get_def //=.
+  rewrite -get_unpack16 //.
+  rewrite pack16K.
+  rewrite get_of_list //.
+  smt().
+  move : i_lb => /#.
+  wp; skip.
+  move => &1 &2 H.
+  split.
+  trivial.
+  trivial.
+qed.
+
+equiv eq_poly_sub:
+  Mprevec.poly_sub ~ Mvec.poly_sub: ={rp, ap, bp} ==> ={res}.
+proof.
+  proc.
+  while(={rp, ap, bp, i} /\ 0 <= i{1}).
+  wp.
+  call eq_iVPSUB_16u16.
+  wp. skip. rewrite /is16u16 => />. move => &1 i_lb i_ub.
+  do split.
+  rewrite /lift2poly; simplify; rewrite pack16_bits16; trivial.
+  rewrite /lift2poly; simplify; rewrite pack16_bits16; trivial.
+  move => ap_eq bp_eq result_L.
+  split.
+  rewrite fillE //=.
+  apply Array256.ext_eq.
+  move => x x_i.
+  have x_mb: 0 <= x %% 16 < 16.
+    by smt().
+  do rewrite initiE //=.
+  rewrite set_get_def //=.
+  rewrite -get_unpack16 //.
+  rewrite pack16K.
+  rewrite get_of_list //.
+  smt().
+  move : i_lb => /#.
+  wp; skip.
+  move => &1 &2 H.
+  split.
+  trivial.
+  trivial.
+qed.
+
+equiv eq_poly_reduce:
+  Mprevec.poly_reduce ~ Mvec.poly_reduce: ={rp} ==> ={res}.
+proof.
+  proc.
+  while(={rp, i} /\ 0 <= i{1} /\ is16u16 qx16{1} qx16{2} /\ is16u16 vx16{1} vx16{2}).
+  inline Mprevec.red16x Mvec.red16x.
+  wp.
+  do !(call eq_iVPSUB_16u16 || call eq_iVPMULL_16u16 || call eq_iVPSRA_16u16 || call eq_iVPMULH_256).
+  wp. skip. rewrite /is16u16 => />. move => &2 i_lb i_ub.
+  do split.
+  rewrite /lift2poly; simplify; rewrite pack16_bits16; trivial.
+  rewrite /lift2poly; simplify; rewrite pack16_bits16; trivial.
+  move => rp_eq res2.
+  do split.
+  rewrite fillE.
+  apply Array256.ext_eq.
+  move => x x_i.
+  do rewrite initiE => />.
+  have x_mb : 0 <= (x %% 16) < 16.
+    move : x_i => /#.
+  rewrite set_get_def => //.
+  rewrite -get_unpack16 => //.
+  rewrite pack16K.
+  rewrite get_of_list => //.
+  smt().
+  move : i_lb => /#.
+  wp; skip.
+  move => &1 &2 rp_eq qx16_R vx16_R qx16_L vx16_L.
+  do split.
+  rewrite rp_eq //=.
+  rewrite /is16u16 /qx16_R /qx16_L /lift2poly;
+  do rewrite initiE => />.
+  rewrite pack16_bits16 => //.
+  rewrite /is16u16 /vx16_R /vx16_L /lift2poly;
+  do rewrite initiE => />.
+  rewrite pack16_bits16 => //.
+  trivial.
+qed.
+
+equiv eq_poly_frommont:
+  Mprevec.poly_frommont ~ Mvec.poly_frommont: ={rp} ==> ={res}.
+proof.
+  proc.
+  while(={rp, i, aux} /\ aux{1} = 16 /\ 0 <= i{1} /\ is16u16 qx16{1} qx16{2} /\ is16u16 qinvx16{1} qinvx16{2} /\ is16u16 dmontx16{1} dmontx16{2}).
+  inline Mprevec.fqmulx16 Mvec.fqmulx16.
+  wp.
+  do !(call eq_iVPSUB_16u16 || call eq_iVPMULH_256 || call eq_iVPMULL_16u16).
+  wp. skip. rewrite /is16u16 => />. move => &2 i_lb i_ub.
+  do split.
+  rewrite /lift2poly initiE => />.
+  rewrite pack16_bits16 => //.
+  move => rp_eq_pack_rp.
+  move => result_L3.
+  split.
+  rewrite fillE.
+  apply Array256.ext_eq.
+  move => x x_i.
+  do rewrite initiE => />.
+  have x_mb : 0 <= (x %% 16) < 16.
+    move : x_i => /#.
+  rewrite set_get_def => //.
+  rewrite -get_unpack16 => //.
+  rewrite pack16K.
+  rewrite get_of_list => //.
+  smt().
+  move : i_lb => /#.
+  wp; skip.
+  move => &1 &2 rp_eq qx16_R qinvx16_R dmontx16_R aux_R qx16_L qinvx16_L dmontx16_L aux_L.
+  split.
+  rewrite rp_eq /=.
+  rewrite /aux_L /aux_R /=.
+  rewrite /is16u16.
+  rewrite /qx16_R /qinvx16_R /dmontx16_R /qx16_L /qinvx16_L /dmontx16_L.
+  rewrite /lift2poly initiE => />.
+  do rewrite pack16_bits16 //.
+  trivial.
+qed.
+
+
+equiv eq_shuffle8:
+  Mprevec.shuffle8 ~ Mvec.shuffle8: is16u16 a{1} a{2} /\ is16u16 b{1} b{2} ==>
+                                    is16u16 res{1}.`1 res{2}.`1 /\
+                                    is16u16 res{1}.`2 res{2}.`2.
+proof.
+  proc.
+  do call eq_iVPERM2I128_16u16.
+  wp; skip; auto => />.
+qed.
+
+equiv eq_shuffle4:
+  Mprevec.shuffle4 ~ Mvec.shuffle4: is16u16 a{1} a{2} /\ is16u16 b{1} b{2} ==>
+                                    is16u16 res{1}.`1 res{2}.`1 /\
+                                    is16u16 res{1}.`2 res{2}.`2.
+proof.
+  proc.
+  call eq_iVPUNPCKH_4u64_16u16.
+  call eq_iVPUNPCKL_4u64_16u16.
+  inline *; wp; skip; auto => />.
+qed.
+
+equiv eq_shuffle2:
+  Mprevec.shuffle2 ~ Mvec.shuffle2: is16u16 a{1} a{2} /\ is16u16 b{1} b{2} ==>
+                                    is16u16 res{1}.`1 res{2}.`1 /\
+                                    is16u16 res{1}.`2 res{2}.`2.
+proof.
+  proc.
+  call eq_iVPBLEND_8u32_16u16.
+  wp.
+  call eq_iVPSRL_4u64.
+  wp.
+  call eq_iVPBLEND_8u32_16u16.
+  call eq_iVMOVSLDUP_256_16u16.
+  inline *; wp; skip; auto => />.
+  move => &1 &2 [#] a_eq b_eq resL resR res_eq resL0 resR0 res0_eq />.
+  split.
+    + by rewrite /is4u64 /f16u16_t4u64.
+    move => aq_eq resL1 resR1 res1_eq />.
+    + rewrite /is16u16 /f4u64_t16u16 res1_eq => />.
+      apply W16u16.allP => />.
+qed.
+
+equiv eq_shuffle1:
+  Mprevec.shuffle1 ~ Mvec.shuffle1: is16u16 a{1} a{2} /\ is16u16 b{1} b{2} ==>
+                                    is16u16 res{1}.`1 res{2}.`1 /\
+                                    is16u16 res{1}.`2 res{2}.`2.
+proof.
+  proc.
+  call eq_iVPBLEND_16u16.
+  wp.
+  call eq_iVPSRL_8u32.
+  wp.
+  call eq_iVPBLEND_16u16.
+  wp.
+  call eq_iVPSLL_8u32.
+  wp.
+  inline *; wp; skip; auto => />.
+  move => &1 &2 [#] a_eq b_eq.
+  split.
+    + by rewrite /is8u32 /f16u16_t8u32.
+    move => bd_eq resL resR res_eq.
+    split.
+    + rewrite /is16u16 /f8u32_t16u16 res_eq => />.
+      apply W16u16.allP => />.
+    move => resd_eq resL0 resR0 res0_eq />.
+    split.
+    + by rewrite /is8u32 /f16u16_t8u32.
+    move => ad_eq resL1 resR1 res1_eq.
+    + rewrite /is16u16 /f8u32_t16u16 res1_eq => />.
+      apply W16u16.allP => />.
+qed.
+
+
+equiv veceq_poly_add2 :
+  Mvec.poly_add2 ~Jkem_avx2.M._poly_add2: ={rp, bp} ==> ={res}.
+proof.
+  proc.
+  while (={rp, bp, i}).
+    inline{1} OpsV.iVPADD_16u16.
+    wp. skip. auto => //.
+  wp. skip. auto => //.
+qed.
+
+
+equiv veceq_poly_sub :
+  Mvec.poly_sub ~Jkem_avx2.M._poly_sub: ={rp, ap, bp} ==> ={res}.
+proof.
+  proc.
+  while (={rp, ap, bp, i}).
+    inline{1} OpsV.iVPSUB_16u16.
+    wp. skip. auto => //.
+  wp. skip. auto => //.
+qed.
+
+equiv veceq_poly_reduce:
+  Mvec.poly_reduce ~Jkem_avx2.M.__poly_reduce: ={rp} ==> ={res}.
+proof.
+  proc.
+  while(={rp, i, qx16, vx16}).
+    inline *.
+    wp. skip. auto => />.
+  wp. skip. auto => />.
+qed.
+
+equiv veceq_poly_frommont:
+  Mvec.poly_frommont ~Jkem_avx2.M._poly_frommont: ={rp} ==> ={res}.
+proof.
+  proc.
+  while(={rp, i, qx16, qinvx16, dmontx16} /\ aux{1} = inc{2}).
+  inline *.
+  wp. skip. auto => />.
+  wp. skip. auto => />.
+qed.
+
+
+equiv veceq_shuffle8:
+  Mvec.shuffle8 ~Jkem_avx2.M.__shuffle8: ={a, b} ==> ={res}.
+proof.
+  proc.
+  inline *; wp; skip; auto => />.
+qed.
+
+equiv veceq_shuffle4:
+  Mvec.shuffle4 ~Jkem_avx2.M.__shuffle4: ={a, b} ==> ={res}.
+proof.
+  proc.
+  inline *; wp; skip; auto => />.
+qed.
+
+equiv veceq_shuffle2:
+  Mvec.shuffle2 ~Jkem_avx2.M.__shuffle2: ={a, b} ==> ={res}.
+proof.
+  proc.
+  inline *; wp; skip; auto => />.
+qed.
+
+equiv veceq_shuffle1:
+  Mvec.shuffle1 ~Jkem_avx2.M.__shuffle1: ={a, b} ==> ={res}.
+proof.
+  proc.
+  inline *; wp; skip; auto => />.
+qed.
+
+
+equiv prevec_eq_poly_add2:
+  Mprevec.poly_add2 ~Jkem_avx2.M._poly_add2: ={rp, bp} ==> ={res}.
+    transitivity Mvec.poly_add2 (={rp, bp} ==> ={res}) (={rp, bp} ==> ={res}).
+smt(). trivial.
+apply eq_poly_add2.
+apply veceq_poly_add2.
+qed.
+
+equiv prevec_eq_poly_sub:
+  Mprevec.poly_sub ~Jkem_avx2.M._poly_sub: ={rp, ap, bp} ==> ={res}.
+    transitivity Mvec.poly_sub (={rp, ap, bp} ==> ={res}) (={rp, ap, bp} ==> ={res}).
+smt(). trivial.
+apply eq_poly_sub.
+apply veceq_poly_sub.
+qed.
+
+equiv prevec_eq_poly_reduce:
+  Mprevec.poly_reduce ~Jkem_avx2.M.__poly_reduce: ={rp} ==> ={res}.
+    transitivity Mvec.poly_reduce (={rp} ==> ={res}) (={rp} ==> ={res}).
+smt(). trivial.
+apply eq_poly_reduce.
+apply veceq_poly_reduce.
+qed.
+
+equiv prevec_eq_poly_frommont:
+  Mprevec.poly_frommont ~Jkem_avx2.M._poly_frommont: ={rp} ==> ={res}.
+    transitivity Mvec.poly_frommont (={rp} ==> ={res}) (={rp} ==> ={res}).
+smt(). trivial.
+apply eq_poly_frommont.
+apply veceq_poly_frommont.
+qed.
+
+
+equiv prevec_eq_shuffle8:
+  Mprevec.shuffle8 ~Jkem_avx2.M.__shuffle8: is16u16 a{1} a{2} /\ is16u16 b{1} b{2} ==>
+                                    is16u16 res{1}.`1 res{2}.`1 /\
+                                    is16u16 res{1}.`2 res{2}.`2.
+proof.
+  transitivity Mvec.shuffle8 (is16u16 a{1} a{2} /\ is16u16 b{1} b{2} ==>
+                              is16u16 res{1}.`1 res{2}.`1 /\
+                              is16u16 res{1}.`2 res{2}.`2)
+                             (={a, b} ==> ={res}).
+  smt(). trivial.
+  apply eq_shuffle8.
+  apply veceq_shuffle8.
+qed.
+
+equiv prevec_eq_shuffle8_sym :
+  Jkem_avx2.M.__shuffle8 ~ Mprevec.shuffle8 : is16u16 a{2} a{1} /\ is16u16 b{2} b{1} ==>
+                                    is16u16 res{2}.`1 res{1}.`1 /\
+                                    is16u16 res{2}.`2 res{1}.`2.
+symmetry. conseq prevec_eq_shuffle8 => />. qed.
+
+equiv prevec_eq_shuffle4:
+  Mprevec.shuffle4 ~Jkem_avx2.M.__shuffle4: is16u16 a{1} a{2} /\ is16u16 b{1} b{2} ==>
+                                    is16u16 res{1}.`1 res{2}.`1 /\
+                                    is16u16 res{1}.`2 res{2}.`2.
+proof.
+  transitivity Mvec.shuffle4 (is16u16 a{1} a{2} /\ is16u16 b{1} b{2} ==>
+                              is16u16 res{1}.`1 res{2}.`1 /\
+                              is16u16 res{1}.`2 res{2}.`2)
+                             (={a, b} ==> ={res}).
+  smt(). trivial.
+  apply eq_shuffle4.
+  apply veceq_shuffle4.
+qed.
+
+equiv prevec_eq_shuffle4_sym:
+  Jkem_avx2.M.__shuffle4 ~ Mprevec.shuffle4: is16u16 a{2} a{1} /\ is16u16 b{2} b{1} ==>
+                                    is16u16 res{2}.`1 res{1}.`1 /\
+                                    is16u16 res{2}.`2 res{1}.`2.
+symmetry. conseq prevec_eq_shuffle4 => />. qed.
+
+equiv prevec_eq_shuffle2:
+  Mprevec.shuffle2 ~Jkem_avx2.M.__shuffle2: is16u16 a{1} a{2} /\ is16u16 b{1} b{2} ==>
+                                    is16u16 res{1}.`1 res{2}.`1 /\
+                                    is16u16 res{1}.`2 res{2}.`2.
+proof.
+  transitivity Mvec.shuffle2 (is16u16 a{1} a{2} /\ is16u16 b{1} b{2} ==>
+                              is16u16 res{1}.`1 res{2}.`1 /\
+                              is16u16 res{1}.`2 res{2}.`2)
+                             (={a, b} ==> ={res}).
+  smt(). trivial.
+  apply eq_shuffle2.
+  apply veceq_shuffle2.
+qed.
+
+equiv prevec_eq_shuffle2_sym:
+  Jkem_avx2.M.__shuffle2 ~ Mprevec.shuffle2 : is16u16 a{2} a{1} /\ is16u16 b{2} b{1} ==>
+                                    is16u16 res{2}.`1 res{1}.`1 /\
+                                    is16u16 res{2}.`2 res{1}.`2.
+symmetry. conseq prevec_eq_shuffle2 => />. qed.
+
+equiv prevec_eq_shuffle1:
+  Mprevec.shuffle1 ~Jkem_avx2.M.__shuffle1: is16u16 a{1} a{2} /\ is16u16 b{1} b{2} ==>
+                                    is16u16 res{1}.`1 res{2}.`1 /\
+                                    is16u16 res{1}.`2 res{2}.`2.
+proof.
+  transitivity Mvec.shuffle1 (is16u16 a{1} a{2} /\ is16u16 b{1} b{2} ==>
+                              is16u16 res{1}.`1 res{2}.`1 /\
+                              is16u16 res{1}.`2 res{2}.`2)
+                             (={a, b} ==> ={res}).
+  smt(). trivial.
+  apply eq_shuffle1.
+  apply veceq_shuffle1.
+qed.
+
+equiv prevec_eq_shuffle1_sym:
+  Jkem_avx2.M.__shuffle1 ~ Mprevec.shuffle1 : is16u16 a{2} a{1} /\ is16u16 b{2} b{1} ==>
+                                    is16u16 res{2}.`1 res{1}.`1 /\
+                                    is16u16 res{2}.`2 res{1}.`2.
+symmetry. conseq prevec_eq_shuffle1 => />. qed.
+
+require import NTT_avx2 NTT_avx2_poly NTT_AVX_j.
+require import.
+
+lemma list_arr16 (x:'a Array16.t):
+  [x.[0];x.[1];x.[2];x.[3];x.[4];x.[5];x.[6];x.[7];x.[8];x.[9];x.[10];x.[11];x.[12];x.[13];x.[14];x.[15]] = to_list x.
+rewrite /to_list /mkseq -iotaredE => />. qed.
+
+lemma avx2_shuffle8_corr_h (_a _b : t16u16) :
+      hoare[ Jkem_avx2.M.__shuffle8 :
+             is16u16 _a a /\ is16u16 _b b
+             ==>
+             is16u16 (NTT_Avx2.shuf8 _a _b).`1 res.`1 /\
+             is16u16 (NTT_Avx2.shuf8 _a _b).`2 res.`2].
+conseq prevec_eq_shuffle8_sym (MLKEM_PolyAVX.shuffle8_corr_h _a _b) => />.
+auto => /> &1 -> ->. exists ((_a,_b)) => />.
+auto => /> &1 &2 -> -> -> ->. rewrite /is16u16 !list_arr16 //. qed.
+
+lemma avx2_shuffle4_corr_h (_a _b : t16u16) :
+      hoare[ Jkem_avx2.M.__shuffle4 :
+             is16u16 _a a /\ is16u16 _b b
+             ==>
+             is16u16 (NTT_Avx2.shuf4 _a _b).`1 res.`1 /\
+             is16u16 (NTT_Avx2.shuf4 _a _b).`2 res.`2].
+conseq prevec_eq_shuffle4_sym (MLKEM_PolyAVX.shuffle4_corr_h _a _b) => />.
+auto => /> &1 -> ->. exists ((_a,_b)) => />.
+auto => /> &1 &2 -> -> -> ->. rewrite /is16u16 !list_arr16 //. qed.
+
+lemma avx2_shuffle2_corr_h (_a _b : t16u16) :
+      hoare[ Jkem_avx2.M.__shuffle2 :
+             is16u16 _a a /\ is16u16 _b b
+             ==>
+             is16u16 (NTT_Avx2.shuf2 _a _b).`1 res.`1 /\
+             is16u16 (NTT_Avx2.shuf2 _a _b).`2 res.`2].
+conseq prevec_eq_shuffle2_sym (MLKEM_PolyAVX.shuffle2_corr_h _a _b) => />.
+auto => /> &1 -> ->. exists ((_a,_b)) => />.
+auto => /> &1 &2 -> -> -> ->. rewrite /is16u16 !list_arr16 //. qed.
+
+lemma avx2_shuffle1_corr_h (_a _b : t16u16) :
+      hoare[ Jkem_avx2.M.__shuffle1 :
+             is16u16 _a a /\ is16u16 _b b
+             ==>
+             is16u16 (NTT_Avx2.shuf1 _a _b).`1 res.`1 /\
+             is16u16 (NTT_Avx2.shuf1 _a _b).`2 res.`2].
+conseq prevec_eq_shuffle1_sym (MLKEM_PolyAVX.shuffle1_corr_h _a _b) => />.
+auto => /> &1 -> ->. exists ((_a,_b)) => />.
+auto => /> &1 &2 -> -> -> ->. rewrite /is16u16 !list_arr16 //. qed.
+
+end MLKEM_PolyAVXVec.
